typing/pure_inference_modelScript.sml
@@ -1,12 +1,17 @@
 
 open HolKernel Parse boolLib bossLib BasicProvers dep_rewrite;
 open pairTheory arithmeticTheory integerTheory stringTheory optionTheory
-     listTheory alistTheory rich_listTheory finite_mapTheory pred_setTheory;
-open pure_typingTheory pure_cexpTheory pure_configTheory pure_varsTheory
-     pure_inference_commonTheory pure_inferenceTheory pure_unificationTheory
+     listTheory alistTheory rich_listTheory finite_mapTheory pred_setTheory
+     sptreeTheory;
+open mlmapTheory;
+open pure_typingTheory pure_typingPropsTheory
+     pure_cexpTheory pure_configTheory pure_varsTheory pure_unificationTheory
+     pure_inference_commonTheory pure_inferenceTheory pure_inferencePropsTheory
      pure_miscTheory;
 
 val _ = new_theory "pure_inference_model";
+
+(******************** Definitions ********************)
 
 Datatype:
   mconstraint = mUnify itype itype
@@ -38,183 +43,22 @@ Definition list_disjoint_def:
     ⇒ DISJOINT mid (BIGUNION (set (left ++ right)))
 End
 
-Theorem list_disjoint_doubleton[simp]:
-  list_disjoint [a;b] ⇔ DISJOINT a b
-Proof
-  rw[list_disjoint_def] >> eq_tac >> rw[]
-  >- (first_x_assum irule >> qexistsl_tac [`[]`] >> simp[]) >>
-  Cases_on `left` >> gvs[] >> Cases_on `t` >> gvs[] >> simp[DISJOINT_SYM]
-QED
-
-Theorem list_disjoint_append:
-  ∀l1 l2. list_disjoint (l1 ++ l2) ⇔
-    list_disjoint l1 ∧ list_disjoint l2 ∧
-    DISJOINT (BIGUNION (set l1)) (BIGUNION (set l2))
-Proof
-  rw[list_disjoint_def] >> eq_tac >> rw[]
-  >- (first_x_assum irule >> qexists_tac `left` >> simp[])
-  >- (first_x_assum irule >> qexists_tac `left` >> simp[])
-  >- (first_x_assum irule >> qexists_tac `l1 ++ left` >> simp[])
-  >- (first_x_assum irule >> qexists_tac `l1 ++ left` >> simp[])
-  >- (
-    first_x_assum irule >> last_x_assum assume_tac >>
-    drule_at Concl $ iffLR MEM_SING_APPEND >> simp[] >> strip_tac >> gvs[] >>
-    qexists_tac `a` >> simp[]
-    )
-  >- (
-    qpat_x_assum `_ ++ _ = _` mp_tac >>
-    simp[APPEND_EQ_APPEND_MID] >> rw[] >> gvs[]
-    >- (last_x_assum irule >> qexists_tac `left` >> simp[])
-    >- (first_x_assum drule >> simp[Once DISJOINT_SYM])
-    >- (last_x_assum kall_tac >> last_x_assum irule >> qexists_tac `l` >> simp[])
-    )
-  >- (
-    qpat_x_assum `_ ++ _ = _` mp_tac >>
-    simp[APPEND_EQ_APPEND_MID] >> rw[] >> gvs[]
-    >- (last_x_assum irule >> qexists_tac `left` >> simp[])
-    >- (last_x_assum kall_tac >> last_x_assum irule >> qexists_tac `l` >> simp[])
-    )
-QED
-
-Theorem TAKE_EL_DROP:
-  ∀n l. n < LENGTH l ⇒
-    l = TAKE n l ++ [EL n l] ++ DROP (SUC n) l
-Proof
-  rw[] >>
-  qspecl_then [`1`,`n`,`l`] assume_tac TAKE_SEG_DROP >> gvs[SEG1, ADD1]
-QED
-
-Theorem list_disjoint_ALL_DISTINCT:
-  ∀l. EVERY FINITE l ⇒
-    (list_disjoint l ⇔ ALL_DISTINCT (FLAT $ MAP SET_TO_LIST l))
-Proof
-  rw[list_disjoint_def, miscTheory.ALL_DISTINCT_FLAT] >>
-  eq_tac >> rw[]
-  >- (gvs[MEM_MAP, EVERY_MEM])
-  >- (
-    gvs[EL_MAP] >>
-    `∃a b c. l = a ++ [EL i l] ++ b ++ [EL j l] ++ c` by (
-      qexistsl_tac [`TAKE i l`,`SEG (j - SUC i) (SUC i) l`,`DROP (SUC j) l`] >>
-      `∃k. j = i + k ∧ 0 < k` by (
-        qpat_x_assum `_ < _` kall_tac >>
-        drule LESS_STRONG_ADD >> rw[] >> simp[]) >>
-      gvs[] >>
-      qspecl_then [`i`,`l`] assume_tac TAKE_EL_DROP >> gvs[] >>
-      first_assum $ (fn th => rewrite_tac[Once th, SimpLHS]) >> simp[] >>
-      once_rewrite_tac[GSYM APPEND_ASSOC] >> rewrite_tac[GSYM CONS_APPEND] >>
-      DEP_REWRITE_TAC[GSYM DROP_CONS_EL] >> simp[SEG_TAKE_DROP, ADD1] >>
-      qspecl_then [`DROP i l`,`1`,`k`] assume_tac $ GSYM DROP_TAKE >>
-      gvs[DROP_DROP_T] >>
-      qspecl_then [`1`,`TAKE k (DROP i l)`,`DROP k (DROP i l)`] assume_tac $
-        GSYM DROP_APPEND >>
-      gvs[] >> `1 - k = 0` by DECIDE_TAC >> pop_assum $ SUBST_ALL_TAC >>
-      gvs[DROP_DROP_T]) >>
-    rename1 `_ ++ [ii] ++ _ ++ [jj] ++ _` >>
-    pop_assum $ SUBST_ALL_TAC >> gvs[] >>
-    first_x_assum $ qspec_then `a` assume_tac >> gvs[] >>
-    pop_assum $ qspec_then `jj` assume_tac >> gvs[DISJOINT_ALT]
-    )
-  >- (
-    gvs[EL_MAP] >> pop_assum mp_tac >> rw[MEM_EL, DISJOINT_ALT] >>
-    first_x_assum $ qspecl_then [`n`,`LENGTH left`] assume_tac >>
-    gvs[EL_APPEND_EQN, EVERY_EL, MEM_SET_TO_LIST] >> CCONTR_TAC >> gvs[]
-    )
-  >- (
-    gvs[EL_MAP] >> pop_assum mp_tac >> rw[MEM_EL, DISJOINT_ALT] >>
-    first_x_assum $ qspecl_then [`LENGTH left`,`LENGTH left + n + 1`] assume_tac >>
-    gvs[EL_APPEND_EQN, EVERY_EL, MEM_SET_TO_LIST] >> CCONTR_TAC >> gvs[]
-    )
-QED
-
-Definition used_vars_constraint_def:
-  used_vars_constraint (mUnify t1 t2) = pure_vars t1 ∪ pure_vars t2 ∧
-  used_vars_constraint (mImplicit t1 vars t2) = vars ∪ pure_vars t1 ∪ pure_vars t2 ∧
-  used_vars_constraint (mInstantiate t (vars, scheme)) = pure_vars t ∪ pure_vars scheme
+Definition new_vars_constraint_def[simp]:
+  new_vars_constraint (mUnify t1 t2) = pure_vars t1 ∪ pure_vars t2 ∧
+  new_vars_constraint (mImplicit t1 vars t2) = pure_vars t1 ∪ pure_vars t2 ∧
+  new_vars_constraint (mInstantiate t (vars, scheme)) = pure_vars t ∪ pure_vars scheme
 End
 
-Definition used_vars_def:
-  used_vars (asms : massumptions) cs ts =
+Definition new_vars_def:
+  new_vars (asms : massumptions) cs t =
     BIGUNION (FRANGE asms) ∪
-    BIGUNION (IMAGE used_vars_constraint cs) ∪
-    BIGUNION (IMAGE pure_vars ts)
+    BIGUNION (IMAGE new_vars_constraint cs) ∪
+    pure_vars t
 End
-
-Theorem massumptions_ok_maunion:
-  ∀as bs.
-    massumptions_ok as ∧ massumptions_ok bs ∧
-    DISJOINT (BIGUNION (FRANGE as)) (BIGUNION (FRANGE bs))
-  ⇒ massumptions_ok (maunion as bs)
-Proof
-  rw[massumptions_ok_def, DISJ_EQ_IMP] >>
-  gvs[IN_FRANGE_FLOOKUP, DOMSUB_FLOOKUP_THM, PULL_EXISTS,
-      maunion_def, FLOOKUP_FMERGE] >> rw[] >>
-  every_case_tac >> gvs[] >> metis_tac[DISJOINT_ALT]
-QED
-
-Theorem BIGUNION_FRANGE_maunion:
-  ∀as bs.
-    BIGUNION (FRANGE (maunion as bs)) =
-    BIGUNION (FRANGE as) ∪ BIGUNION (FRANGE bs)
-Proof
-  rw[] >> once_rewrite_tac[EXTENSION] >>
-  rw[] >> eq_tac >> rw[] >>
-  gvs[IN_FRANGE_FLOOKUP, PULL_EXISTS, maunion_def, FLOOKUP_FMERGE]
-  >- (every_case_tac >> gvs[] >> metis_tac[])
-  >- (
-    Cases_on `FLOOKUP bs k` >> gvs[]
-    >- (goal_assum drule >> qexists_tac `k` >> simp[])
-    >- (qexistsl_tac [`s ∪ x'`,`k`] >> simp[])
-    )
-  >- (
-    Cases_on `FLOOKUP as k` >> gvs[]
-    >- (goal_assum drule >> qexists_tac `k` >> simp[])
-    >- (qexistsl_tac [`s ∪ x'`,`k`] >> simp[UNION_COMM])
-    )
-QED
 
 Definition cvars_disjoint_def:
-  cvars_disjoint l ⇔ list_disjoint (MAP (λ(as,cs,t). used_vars as cs {t}) l)
+  cvars_disjoint l ⇔ list_disjoint (MAP (λ(as,cs,t). new_vars as cs t) l)
 End
-
-(* TODO delete
-Definition massumptions_list_ok_def:
-  massumptions_list_ok (asms : massumptions list) ⇔
-    EVERY massumptions_ok asms ∧
-    (* each assumption k |-> x has x unique within the list *)
-    ∀left mid right x.
-      asms = left ++ [mid] ++ right ∧
-      x ∈ BIGUNION (FRANGE mid)
-    ⇒ x ∉ BIGUNION $ set (MAP (BIGUNION o FRANGE) (left ++ right))
-End
-
-Theorem massumptions_list_ok_remove:
-  ∀al a ar.
-    massumptions_list_ok (al ++ [a] ++ ar) ⇒ massumptions_list_ok (al ++ ar)
-Proof
-  rw[massumptions_list_ok_def, DISJ_EQ_IMP] >>
-  gvs[combinTheory.o_DEF, MEM_MAP] >> rw[] >>
-  gvs[PULL_EXISTS, PULL_FORALL, AND_IMP_INTRO, IMP_CONJ_THM] >>
-  gvs[FORALL_AND_THM, PULL_EXISTS, GSYM CONJ_ASSOC] >>
-  qpat_x_assum `_ ++ _ = _` mp_tac >>
-  simp[APPEND_EQ_APPEND_MID] >> rw[] >> gvs[]
-  >- (
-    first_x_assum $ qspec_then `left` mp_tac >> gvs[] >>
-    rpt $ disch_then $ drule_at $ Pos last >> simp[]
-    )
-  >- (
-    first_x_assum $ qspec_then `al ++ [a] ++ l` mp_tac >> gvs[] >>
-    rpt $ disch_then $ drule_at $ Pos last >> simp[]
-    )
-  >- (
-    last_x_assum $ qspec_then `left` mp_tac >> gvs[] >>
-    rpt $ disch_then $ drule_at $ Pos last >> simp[]
-    )
-  >- (
-    last_x_assum $ qspec_then `al ++ [a] ++ l` mp_tac >> gvs[] >>
-    rpt $ disch_then $ drule_at $ Pos last >> simp[]
-    )
-QED
-*)
 
 Inductive minfer:
 [~Var:]
@@ -240,8 +84,8 @@ Inductive minfer:
   (minfer ns mset e1 as1 cs1 ty1 ∧
    minfer ns mset e2 as2 cs2 ty2 ∧
    cvars_disjoint [(as1,cs1,ty1);(as2,cs2,ty2)] ∧
-   f1 ∉ mset ∪ used_vars (maunion as1 as2) (cs1 ∪ cs2) {ty1;ty2} ∧
-   f2 ∉ mset ∪ used_vars (maunion as1 as2) (cs1 ∪ cs2) {ty1;ty2}
+   f1 ∉ mset ∪ new_vars as1 cs1 ty1 ∪ new_vars as2 cs2 ty2 ∧
+   f2 ∉ mset ∪ new_vars as1 cs1 ty1 ∪ new_vars as2 cs2 ty2
     ⇒ minfer ns mset (Prim d (Cons "Bind") [e1;e2])
         (maunion as1 as2)
         ({mUnify ty1 (M $ CVar f1); mUnify ty2 (Function (CVar f1) (M $ CVar f2))}
@@ -250,7 +94,7 @@ Inductive minfer:
 
 [~Raise:]
   (minfer ns mset e as cs ty ∧
-   f ∉ mset ∪ used_vars as cs {ty}
+   f ∉ mset ∪ new_vars as cs ty
     ⇒ minfer ns mset (Prim d (Cons "Raise") [e])
         as (mUnify ty Exception INSERT cs) (M $ CVar f)) ∧
 
@@ -258,8 +102,8 @@ Inductive minfer:
   (minfer ns mset e1 as1 cs1 ty1 ∧
    minfer ns mset e2 as2 cs2 ty2 ∧
    cvars_disjoint [(as1,cs1,ty1);(as2,cs2,ty2)] ∧
-   f1 ∉ mset ∪ used_vars (maunion as1 as2) (cs1 ∪ cs2) {ty1; ty2} ∧
-   f2 ∉ mset ∪ used_vars (maunion as1 as2) (cs1 ∪ cs2) {ty1; ty2}
+   f1 ∉ mset ∪ new_vars as1 cs1 ty1 ∪ new_vars as2 cs2 ty2 ∧
+   f2 ∉ mset ∪ new_vars as1 cs1 ty1 ∪ new_vars as2 cs2 ty2
     ⇒ minfer ns mset (Prim d (Cons "Handle") [e1;e2])
         (maunion as1 as2)
         ({mUnify ty1 (M $ CVar f1); mUnify ty2 (Function Exception (M $ CVar f2))}
@@ -282,7 +126,7 @@ Inductive minfer:
 
 [~Length:]
   (minfer ns mset e as cs ty ∧
-   f ∉ mset ∪ used_vars as cs {ty}
+   fresh ∉ mset ∪ new_vars as cs ty
     ⇒ minfer ns mset (Prim d (Cons "Length") [e])
         as (mUnify ty (Array $ CVar fresh) INSERT cs) (M IntTy)) ∧
 
@@ -290,7 +134,7 @@ Inductive minfer:
   (minfer ns mset e1 as1 cs1 ty1 ∧
    minfer ns mset e2 as2 cs2 ty2 ∧
    cvars_disjoint [(as1,cs1,ty1);(as2,cs2,ty2)] ∧
-   f ∉ mset ∪ used_vars (maunion as1 as2) (cs1 ∪ cs2) {ty1;ty2}
+   f ∉ mset ∪ new_vars as1 cs1 ty1 ∪ new_vars as2 cs2 ty2
     ⇒ minfer ns mset (Prim d (Cons "Deref") [e1;e2])
         (maunion as1 as2)
         ({mUnify ty2 IntTy; mUnify ty1 (Array $ CVar f)} ∪ cs1 ∪ cs2)
@@ -301,7 +145,7 @@ Inductive minfer:
    minfer ns mset e2 as2 cs2 ty2 ∧
    minfer ns mset e3 as3 cs3 ty3 ∧
    cvars_disjoint [(as1,cs1,ty1);(as2,cs2,ty2);(as3,cs3,ty3)] ∧
-   f ∉ mset ∪ used_vars as (cs1 ∪ cs2 ∪ cs3) {ty1;ty2;ty3}
+   f ∉ mset ∪ new_vars as1 cs1 ty1 ∪ new_vars as2 cs2 ty2 ∪ new_vars as3 cs3 ty3
     ⇒ minfer ns mset (Prim d (Cons "Update") [e1;e2;e3])
         as
         ({mUnify ty3 (CVar f); mUnify ty2 IntTy; mUnify ty1 (Array $ CVar f)}
@@ -340,13 +184,13 @@ Inductive minfer:
    ALOOKUP cns cname = SOME arg_tys ∧
    LENGTH arg_tys = LENGTH tys ∧
    LENGTH freshes = ar ∧
-   EVERY (λf.
-    f ∉ mset ∪ used_vars (FOLDR maunion FEMPTY ass) (BIGUNION (set css)) (set tys))
-      freshes ∧
+   EVERY (λf. f ∉ mset ∧
+    EVERY (λ(as,cs,ty). f ∉ new_vars as cs ty) (ZIP (ass,ZIP(css,tys)))) freshes ∧
    s ∉ reserved_cns
     ⇒ minfer ns mset (Prim d (Cons s) es)
         (FOLDR maunion FEMPTY ass)
-        (set (list$MAP2 (λt a. mUnify t (isubst cfreshes $ itype_of a)) tys arg_tys) ∪
+        (set (list$MAP2
+              (λt a. mUnify t (isubst (MAP CVar freshes) $ itype_of a)) tys arg_tys) ∪
           BIGUNION (set css))
         (TypeCons id (MAP CVar freshes))) ∧
 
@@ -376,9 +220,10 @@ Inductive minfer:
       (ZIP (es,tys)) (ZIP (ass,css)) ∧
    minfer ns mset e fas fcs fty ∧
    cvars_disjoint ((fas,fcs,fty)::ZIP (ass, ZIP (css, tys))) ∧
+   f ∉ mset ∧
+   EVERY (λ(as,cs,ty). f ∉ new_vars as cs ty) (ZIP (fas::ass,ZIP(fcs::css,fty::tys))) ∧
    as = FOLDR maunion FEMPTY (fas::ass) ∧
-   cs = fcs ∪ BIGUNION (set css) ∧
-   f ∉ mset ∪ used_vars as cs (fty INSERT set tys)
+   cs = fcs ∪ BIGUNION (set css)
     ⇒ minfer ns mset (App d e es)
         as (mUnify fty (iFunctions tys (CVar f)) INSERT cs) (CVar f)) ∧
 
@@ -386,7 +231,7 @@ Inductive minfer:
   (¬NULL xs ∧
    minfer ns (set freshes ∪ mset) e as cs ty ∧
    LENGTH freshes = LENGTH xs ∧
-   EVERY (λf. f ∉ mset ∪ used_vars as cs {ty}) freshes
+   EVERY (λf. f ∉ mset ∪ new_vars as cs ty) freshes
     ⇒ minfer ns mset (Lam d xs e)
         (FDIFF as (set xs))
         (cs ∪ (BIGUNION $ set $ list$MAP2 (λf x.
@@ -420,51 +265,1918 @@ Inductive minfer:
 [~TupleCase:]
   (¬MEM v pvars ∧
    minfer ns (f INSERT set freshes ∪ mset) rest asrest csrest tyrest ∧
-   minfer ns mset rest eas ecs ety ∧
-   f ∉ mset ∪ used_vars (maunion eas asrest) (ecs ∪ csrest) {ety; tyrest} ∧
+   minfer ns mset e eas ecs ety ∧
    EVERY (λf.
-    f ∉ mset ∪ used_vars (maunion eas asrest) (ecs ∪ csrest) {ety; tyrest})
-    freshes ∧
+    f ∉ mset ∪ new_vars eas ecs ety ∪ new_vars asrest csrest tyrest)
+    (f::freshes) ∧
    pvar_cs =
     list$MAP2
       (λv t. IMAGE (λn. mUnify (CVar n) t) (get_massumptions asrest v))
       (v::pvars) (MAP CVar $ f::freshes)
     ⇒ minfer ns mset (Case d e v [("",pvars,rest)])
         (maunion as (FDIFF asrest (set (v::pvars))))
-        (mUnify (CVar f) tye INSERT mUnify tye (Tuple $ MAP CVar freshes) INSERT
+        (mUnify (CVar f) ety INSERT mUnify ety (Tuple $ MAP CVar freshes) INSERT
           BIGUNION (set pvar_cs) ∪ cs)
         tyrest) ∧
 
 [~Case:]
   (¬MEM v (FLAT (MAP (FST o SND) cases)) ∧
-   get_typedef 0 (SND ns)
-    (MAP (λ(cn,pvs,_). (cn, LENGTH pvs)) cases) = SOME (id, ar, cdefs) ∧
-   expected_arg_tys =
-    MAP (λ(cn,ts). (cn, MAP (isubst (MAP CVar freshes) o itype_of) ts)) cdefs ∧
+   oEL id (SND ns) = SOME (ar, cdefs) ∧
+   PERM (MAP (λ(cn,ts). (cn, LENGTH ts)) cdefs)
+    (MAP (λ(cn,pvars,rest). (cn, LENGTH pvars)) cases) ∧
    LENGTH cases = LENGTH tys ∧
    LENGTH ass = LENGTH css ∧
    LIST_REL (λ((cname,pvars,rest),ty) (a,c).
-      ∃asrest csrest.
-        minfer ns (f INSERT set freshes ∪ mset) rest asrest csrest ty ∧
-        ALOOKUP expected_arg_tys cname = SOME expected_cname_arg_tys ∧
-        let pvar_cs = list$MAP2
-          (λv t. IMAGE (λn. mUnify (CVar n) t) (get_massumptions asrest v))
-          (v::pvars) (CVar f :: expected_cname_arg_tys) in
-        a = FDIFF asrest (v INSERT set pvars) ∧
-        c = BIGUNION (set pvar_cs) ∪ csrest)
+      minfer ns (f INSERT set freshes ∪ mset) rest a c ty)
       (ZIP (cases,tys)) (ZIP (ass,css)) ∧
    minfer ns mset e eas ecs ety ∧
    cvars_disjoint ((eas,ecs,ety)::ZIP (ass, ZIP (css, tys))) ∧
-   as = FOLDR maunion FEMPTY (eas::ass) ∧
-   cs = ecs ∪ BIGUNION (set css) ∧
-   f ∉ mset ∪ used_vars as cs (ety INSERT set tys) ∧
-   EVERY (λf.  f ∉ mset ∪ used_vars as cs (ety INSERT set tys)) freshes
+   EVERY (λf. f ∉ mset ∧
+    EVERY (λ(as,cs,ty). f ∉ new_vars as cs ty)
+      (ZIP (eas::ass,ZIP(ecs::css,ety::tys)))) (f::freshes) ∧
+   LENGTH final_as = LENGTH final_cs ∧
+   LIST_REL (λ((cn,pvars,rest),as,cs) (as',cs').
+    ∃schemes.
+      ALOOKUP cdefs cn = SOME schemes ∧
+      let pvar_cs = list$MAP2
+        (λv t. IMAGE (λn. mUnify (CVar n) t) (get_massumptions as v))
+        (v::pvars) (CVar f :: MAP (isubst (MAP CVar freshes) o itype_of) schemes) in
+      as' = FDIFF as (v INSERT set pvars) ∧
+      cs' = BIGUNION (set pvar_cs) ∪ cs)
+    (ZIP (cases,ZIP (ass,css))) (ZIP (final_as,final_cs))
     ⇒ minfer ns mset (Case d e v cases)
-        as
-        (mUnify (CVar f) tye INSERT mUnify tye (TypeCons id (MAP CVar freshes)) INSERT
-          set (MAP (λt. mUnify (HD tys) t) (TL tys)) ∪ cs)
+        (FOLDR maunion FEMPTY (eas::final_as))
+        (mUnify (CVar f) ety INSERT mUnify ety (TypeCons id (MAP CVar freshes)) INSERT
+          set (MAP (λt. mUnify (HD tys) t) (TL tys)) ∪ ecs ∪ BIGUNION (set final_cs))
         (HD tys))
 End
+
+
+(******************** Proof apparatus ********************)
+
+Definition to_mconstraint_def[simp]:
+  to_mconstraint (Unify d t1 t2) = mUnify t1 t2 ∧
+  to_mconstraint (Instantiate d t sch) = mInstantiate t sch ∧
+  to_mconstraint (Implicit d t1 mono t2) = mImplicit t1 (domain mono) t2
+End
+
+Definition assumptions_rel_def:
+  assumptions_rel asms masms ⇔
+    map_ok asms ∧ cmp_of asms = var_cmp ∧
+    (∀s. FLOOKUP masms s = OPTION_MAP domain (lookup asms s)) ∧
+    (∀s aset. lookup asms s = SOME aset ⇒ wf aset)
+End
+
+
+(******************** Lemmas ********************)
+
+Triviality maunion_comm:
+  ∀x y. maunion x y = maunion y x
+Proof
+  rw[maunion_def] >>
+  irule $ iffRL $ SIMP_RULE (srw_ss()) [combinTheory.COMM_DEF] FMERGE_COMM >>
+  rw[UNION_COMM]
+QED
+
+Theorem list_disjoint_alt_def:
+  list_disjoint l ⇔
+    ∀left right. l = left ++ right ⇒
+      DISJOINT (BIGUNION (set left)) (BIGUNION (set right))
+Proof
+  rw[list_disjoint_def] >> eq_tac >> rw[]
+  >- (
+    first_x_assum irule >>
+    qspecl_then [`left`,`s'`] assume_tac $ GEN_ALL MEM_SING_APPEND >> gvs[] >>
+    qexists_tac `a` >> simp[]
+    )
+  >- (
+    once_rewrite_tac[DISJOINT_SYM] >>
+    first_x_assum irule >> qexists_tac `left` >> simp[]
+    )
+  >- (first_x_assum irule >> qexists_tac `left ++ [mid]` >> simp[])
+QED
+
+Theorem list_disjoint_singleton[simp]:
+  list_disjoint [a]
+Proof
+  rw[list_disjoint_alt_def] >> Cases_on `left` >> gvs[]
+QED
+
+Theorem list_disjoint_doubleton[simp]:
+  list_disjoint [a;b] ⇔ DISJOINT a b
+Proof
+  rw[list_disjoint_def] >> eq_tac >> rw[]
+  >- (first_x_assum irule >> qexistsl_tac [`[]`] >> simp[]) >>
+  Cases_on `left` >> gvs[] >> Cases_on `t` >> gvs[] >> simp[DISJOINT_SYM]
+QED
+
+Theorem list_disjoint_append:
+  ∀l1 l2. list_disjoint (l1 ++ l2) ⇔
+    list_disjoint l1 ∧ list_disjoint l2 ∧
+    DISJOINT (BIGUNION (set l1)) (BIGUNION (set l2))
+Proof
+  rw[list_disjoint_alt_def] >> eq_tac >> rw[]
+  >- (first_x_assum irule >> qexists_tac `left` >> simp[])
+  >- (first_x_assum irule >> qexists_tac `l1 ++ left` >> simp[])
+  >- (first_x_assum irule >> qexists_tac `l1` >> simp[]) >>
+  gvs[APPEND_EQ_APPEND]
+  >- (last_x_assum irule >> ntac 2 $ goal_assum drule >> simp[])
+  >- (
+    last_x_assum kall_tac >> last_x_assum irule >>
+    ntac 2 $ goal_assum drule >> simp[]
+    )
+QED
+
+Theorem list_disjoint_ALL_DISTINCT:
+  ∀l. EVERY FINITE l ⇒
+    (list_disjoint l ⇔ ALL_DISTINCT (FLAT $ MAP SET_TO_LIST l))
+Proof
+  rw[list_disjoint_alt_def, miscTheory.ALL_DISTINCT_FLAT] >>
+  eq_tac >> rw[]
+  >- (gvs[MEM_MAP, EVERY_MEM])
+  >- (
+    gvs[EL_MAP] >> pop_assum mp_tac >>
+    DEP_REWRITE_TAC[MEM_SET_TO_LIST] >> conj_tac >- gvs[EVERY_EL] >>
+    qid_spec_tac `e` >> simp[GSYM DISJOINT_ALT] >>
+    first_x_assum irule >>
+    qexistsl_tac [`TAKE (SUC i) l`,`DROP (SUC i) l`] >> rw[MEM_EL]
+    >- (qexists_tac `i` >> simp[EL_TAKE])
+    >- (qexists_tac `j - SUC i` >> simp[EL_DROP])
+    )
+  >- (
+    gvs[EL_MAP] >> ntac 2 $ pop_assum mp_tac >> rw[MEM_EL] >>
+    first_x_assum $ qspecl_then [`n`,`LENGTH left + n'`] assume_tac >> gvs[] >>
+    rw[DISJOINT_ALT] >> first_x_assum $ qspec_then `x` mp_tac >>
+    simp[EL_APPEND_EQN] >>
+    DEP_REWRITE_TAC[MEM_SET_TO_LIST] >> simp[] >> gvs[EVERY_EL]
+    )
+QED
+
+Theorem massumptions_ok_maunion:
+  ∀as bs.
+    massumptions_ok as ∧ massumptions_ok bs ∧
+    DISJOINT (BIGUNION (FRANGE as)) (BIGUNION (FRANGE bs))
+  ⇒ massumptions_ok (maunion as bs)
+Proof
+  rw[massumptions_ok_def, DISJ_EQ_IMP] >>
+  gvs[IN_FRANGE_FLOOKUP, DOMSUB_FLOOKUP_THM, PULL_EXISTS,
+      maunion_def, FLOOKUP_FMERGE] >> rw[] >>
+  every_case_tac >> gvs[] >> metis_tac[DISJOINT_ALT]
+QED
+
+Theorem BIGUNION_FRANGE_maunion:
+  ∀as bs.
+    BIGUNION (FRANGE (maunion as bs)) =
+    BIGUNION (FRANGE as) ∪ BIGUNION (FRANGE bs)
+Proof
+  rw[] >> once_rewrite_tac[EXTENSION] >>
+  rw[] >> eq_tac >> rw[] >>
+  gvs[IN_FRANGE_FLOOKUP, PULL_EXISTS, maunion_def, FLOOKUP_FMERGE]
+  >- (every_case_tac >> gvs[] >> metis_tac[])
+  >- (
+    Cases_on `FLOOKUP bs k` >> gvs[]
+    >- (goal_assum drule >> qexists_tac `k` >> simp[])
+    >- (qexistsl_tac [`s ∪ x'`,`k`] >> simp[])
+    )
+  >- (
+    Cases_on `FLOOKUP as k` >> gvs[]
+    >- (goal_assum drule >> qexists_tac `k` >> simp[])
+    >- (qexistsl_tac [`s ∪ x'`,`k`] >> simp[UNION_COMM])
+    )
+QED
+
+Theorem LIST_TO_SET_get_assumptions:
+  ∀as mas. assumptions_rel as mas ⇒
+    ∀x. set (get_assumptions x as) = get_massumptions mas x
+Proof
+  rw[EXTENSION, get_assumptions_def, get_massumptions_def] >>
+  gvs[assumptions_rel_def] >> CASE_TAC >> gvs[] >>
+  simp[miscTheory.toAList_domain]
+QED
+
+Triviality domain_list_insert_alt:
+  domain (list_insert xs t) = set xs ∪ domain t
+Proof
+  rw[EXTENSION, domain_list_insert]
+QED
+
+Theorem FLOOKUP_FOLDR_maunion:
+  ∀ms base k.
+    FLOOKUP (FOLDR maunion base ms) k =
+      if k ∉ FDOM base ∧ ∀m. MEM m ms ⇒ k ∉ FDOM m then NONE
+      else  SOME $
+        BIGUNION {s | FLOOKUP base k = SOME s ∨ ∃m. MEM m ms ∧ FLOOKUP m k = SOME s}
+Proof
+  Induct >> rw[]
+  >- simp[FLOOKUP_DEF]
+  >- simp[FLOOKUP_DEF]
+  >- (gvs[maunion_def, FLOOKUP_FMERGE] >> gvs[FLOOKUP_DEF]) >>
+  gvs[maunion_def, FLOOKUP_FMERGE] >> gvs[FLOOKUP_DEF] >>
+  every_case_tac >> gvs[] >> rw[EXTENSION] >> metis_tac[]
+QED
+
+Triviality infer_bind_alt_def:
+  ∀g f.
+    infer_bind g f = λs. case g s of NONE => NONE | SOME ((a,b,c),s') => f (a,b,c) s'
+Proof
+  rw[FUN_EQ_THM, infer_bind_def] >> rpt (CASE_TAC >> simp[])
+QED
+
+val inferM_ss = simpLib.named_rewrites "inferM_ss"
+  [infer_bind_alt_def, infer_bind_def, infer_ignore_bind_def, fail_def,
+   return_def, fresh_var_def, fresh_vars_def, oreturn_def];
+
+val _ = simpLib.register_frag inferM_ss;
+
+val inferM_rws = SF inferM_ss;
+
+Theorem infer_minfer:
+  ∀ns mset e n ty as cs m.
+    infer ns mset e n = SOME ((ty,as,cs),m) ∧
+    namespace_ok ns ∧
+    (∀mvar. mvar ∈ domain mset ⇒ mvar < n) ⇒
+    ∃mas.
+      assumptions_rel as mas ∧
+      minfer ns (domain mset) e mas (set (MAP to_mconstraint cs)) ty ∧
+      n ≤ m ∧
+      (new_vars mas (set (MAP to_mconstraint cs)) ty ⊆ { v | n ≤ v ∧ v < m})
+Proof
+  recInduct infer_ind >> rw[infer_def]
+  >- ( (* Var *)
+    last_x_assum mp_tac >> rw[inferM_rws] >>
+    qexists_tac `FEMPTY |+ (x, {n})` >> simp[assumptions_rel_def] >>
+    simp[lookup_singleton, FLOOKUP_UPDATE] >> rw[]
+    >- simp[wf_insert]
+    >- (
+      simp[Once minfer_cases] >> CCONTR_TAC >> gvs[] >>
+      last_x_assum drule >> simp[]
+      )
+    >- gvs[new_vars_def, pure_vars]
+    )
+  >- ( (* Tuple *)
+    gvs[inferM_rws] >> every_case_tac >> gvs[] >> pairarg_tac >> gvs[] >>
+    ntac 2 $ pop_assum mp_tac >>
+    map_every qid_spec_tac [`m`,`n`,`tys`,`as`,`cs`] >>
+    Induct_on `es` >> rw[] >> simp[]
+    >- (
+      qexists_tac `FEMPTY` >> simp[assumptions_rel_def] >>
+      simp[Once minfer_cases, PULL_EXISTS] >>
+      qexistsl_tac [`[]`,`[]`] >> simp[cvars_disjoint_def, new_vars_def] >>
+      simp[list_disjoint_def, pure_vars]
+      ) >>
+    every_case_tac >> gvs[] >>
+    last_x_assum drule >> strip_tac >> gvs[] >>
+    last_x_assum $ qspec_then `h` mp_tac >> simp[] >>
+    disch_then drule >> impl_tac >- (rw[] >> first_x_assum drule >> rw[]) >>
+    strip_tac >> gvs[] >> qexists_tac `maunion mas' mas` >> rw[]
+    >- (
+      gvs[assumptions_rel_def, aunion_def, PULL_FORALL] >> rpt gen_tac >>
+      DEP_REWRITE_TAC[cj 1 unionWith_thm, cj 2 unionWith_thm, lookup_unionWith] >>
+      simp[maunion_def, FLOOKUP_FMERGE] >>
+      every_case_tac >> gvs[] >> rw[] >>
+      once_rewrite_tac[UNION_COMM] >> metis_tac[wf_union, domain_union]
+      )
+    >- (
+      qpat_x_assum `minfer _ _ _ _ _ (Tuple _)` mp_tac >>
+      once_rewrite_tac[minfer_cases] >> simp[] >> strip_tac >> gvs[] >>
+      rename1 `set (_ cs) ∪ _` >>
+      qexistsl_tac [`mas'::ass`, `(set (MAP to_mconstraint cs)) :: css`] >>
+      gvs[cvars_disjoint_def] >>
+      once_rewrite_tac[CONS_APPEND] >> rewrite_tac[list_disjoint_append] >>
+      simp[MEM_MAP, EXISTS_PROD, PULL_EXISTS] >> rpt gen_tac >>
+      DEP_REWRITE_TAC[MEM_ZIP] >> DEP_REWRITE_TAC[cj 1 LENGTH_ZIP] >> simp[] >>
+      imp_res_tac LIST_REL_LENGTH >> gvs[] >> simp[PULL_EXISTS] >> rw[] >>
+      pop_assum mp_tac >> DEP_REWRITE_TAC[EL_ZIP] >> simp[] >> strip_tac >> gvs[] >>
+      irule SUBSET_DISJOINT >>
+      qexistsl_tac [`{v | r ≤ v ∧ v < m}`,`{v | n ≤ v ∧ v < r}`] >>
+      conj_tac >- rw[DISJOINT_ALT] >> gvs[] >>
+      irule SUBSET_TRANS >> goal_assum $ drule_at Any >>
+      simp[new_vars_def, BIGUNION_SUBSET, pure_vars, PULL_EXISTS] >> rw[]
+      >- (
+        simp[SUBSET_DEF] >> rw[] >> ntac 2 disj1_tac >>
+        gvs[IN_FRANGE_FLOOKUP, FLOOKUP_FOLDR_maunion, PULL_EXISTS,
+            GSYM CONJ_ASSOC, FLOOKUP_DEF] >>
+        rpt $ goal_assum $ drule_at Any >> simp[EL_MEM]
+        )
+      >- (
+        simp[SUBSET_DEF] >> rw[] >> disj1_tac >> disj2_tac >>
+        simp[PULL_EXISTS] >> rpt $ goal_assum drule >> simp[EL_MEM]
+        )
+      >- (
+        simp[SUBSET_DEF] >> rw[] >> disj2_tac >> simp[MEM_MAP, PULL_EXISTS] >>
+        goal_assum drule >> simp[EL_MEM]
+        )
+      )
+    >- (
+      gvs[new_vars_def, BIGUNION_FRANGE_maunion, GSYM CONJ_ASSOC, pure_vars] >> rw[] >>
+      rename1 `foo ⊆ _` >> gvs[SUBSET_DEF] >> rw[] >> first_x_assum drule >> rw[]
+      )
+    )
+  >- ( (* Ret *)
+    gvs[inferM_rws] >> Cases_on `es` >> gvs[] >> Cases_on `t` >> gvs[inferM_rws] >>
+    every_case_tac >> gvs[] >>
+    last_x_assum drule_all >> strip_tac >> simp[] >>
+    goal_assum drule >> simp[Once minfer_cases] >>
+    gvs[new_vars_def, pure_vars]
+    )
+  >- ( (* Bind *)
+    gvs[inferM_rws] >>
+    Cases_on `es` >> gvs[] >> Cases_on `t` >> gvs[] >>
+    Cases_on `t'` >> gvs[inferM_rws] >> every_case_tac >> gvs[] >>
+    first_x_assum drule_all >> strip_tac >> gvs[] >>
+    last_x_assum drule >> impl_tac
+    >- (rw[] >> last_x_assum drule >> simp[]) >>
+    strip_tac >> gvs[] >>
+    simp[Once minfer_cases, PULL_EXISTS] >>
+    ntac 2 $ goal_assum $ drule_at Any >> qexists_tac `r'` >> rw[]
+    >- (
+      gvs[assumptions_rel_def] >> simp[PULL_FORALL, aunion_def] >>
+      rpt gen_tac >> DEP_REWRITE_TAC[lookup_unionWith] >>
+      DEP_REWRITE_TAC[cj 1 unionWith_thm, cj 2 unionWith_thm] >> simp[] >>
+      simp[maunion_def, FLOOKUP_FMERGE] >>
+      every_case_tac >> gvs[] >> rw[] >>
+      metis_tac[wf_union, domain_union]
+      )
+    >- (rw[EXTENSION] >> eq_tac >> rw[] >> simp[])
+    >- (
+      simp[cvars_disjoint_def, DISJOINT_ALT] >> rw[] >> CCONTR_TAC >> gvs[SUBSET_DEF] >>
+      first_x_assum drule >> strip_tac >> first_x_assum drule >> strip_tac >> gvs[]
+      )
+    >- (CCONTR_TAC >> gvs[] >> first_x_assum drule >> simp[])
+    >- (CCONTR_TAC >> gvs[SUBSET_DEF] >> first_x_assum drule >> simp[])
+    >- (CCONTR_TAC >> gvs[SUBSET_DEF] >> first_x_assum drule >> simp[])
+    >- (CCONTR_TAC >> gvs[] >> first_x_assum drule >> simp[])
+    >- (CCONTR_TAC >> gvs[SUBSET_DEF] >> first_x_assum drule >> simp[])
+    >- (CCONTR_TAC >> gvs[SUBSET_DEF] >> first_x_assum drule >> simp[])
+    >- (
+      gvs[new_vars_def, BIGUNION_FRANGE_maunion, GSYM CONJ_ASSOC] >>
+      simp[new_vars_constraint_def, pure_vars] >>
+      rw[] >> rename1 `foo ⊆ _` >> gvs[SUBSET_DEF] >> rw[] >>
+      first_x_assum drule >> rw[]
+      )
+    )
+  >- ( (* Raise *)
+    gvs[inferM_rws] >>
+    Cases_on `es` >> gvs[] >> Cases_on `t` >> gvs[] >> every_case_tac >> gvs[] >>
+    first_x_assum drule_all >> strip_tac >> gvs[] >>
+    goal_assum drule >> simp[Once minfer_cases, PULL_EXISTS, GSYM CONJ_ASSOC] >>
+    goal_assum $ drule_at Any >> simp[] >> rw[]
+    >- (CCONTR_TAC >> gvs[] >> first_x_assum drule >> simp[])
+    >- (CCONTR_TAC >> gvs[SUBSET_DEF] >> first_x_assum drule >> simp[]) >>
+    gvs[new_vars_def, new_vars_constraint_def, pure_vars] >>
+    rw[] >> rename1 `foo ⊆ _` >> gvs[SUBSET_DEF] >> rw[] >>
+    first_x_assum drule >> rw[]
+    )
+  >- ( (* Handle *)
+    gvs[inferM_rws] >>
+    Cases_on `es` >> gvs[] >> Cases_on `t` >> gvs[] >>
+    Cases_on `t'` >> gvs[inferM_rws] >> every_case_tac >> gvs[] >>
+    first_x_assum drule_all >> strip_tac >> gvs[] >>
+    last_x_assum drule >> impl_tac
+    >- (rw[] >> last_x_assum drule >> simp[]) >>
+    strip_tac >> gvs[] >>
+    simp[Once minfer_cases, PULL_EXISTS] >>
+    ntac 2 $ goal_assum $ drule_at Any >> qexists_tac `r'` >> rw[]
+    >- (
+      gvs[assumptions_rel_def] >> simp[PULL_FORALL, aunion_def] >>
+      rpt gen_tac >> DEP_REWRITE_TAC[lookup_unionWith] >>
+      DEP_REWRITE_TAC[cj 1 unionWith_thm, cj 2 unionWith_thm] >> simp[] >>
+      simp[maunion_def, FLOOKUP_FMERGE] >>
+      every_case_tac >> gvs[] >> rw[] >>
+      metis_tac[wf_union, domain_union]
+      )
+    >- (rw[EXTENSION] >> eq_tac >> rw[] >> simp[])
+    >- (
+      simp[cvars_disjoint_def, DISJOINT_ALT] >> rw[] >> CCONTR_TAC >> gvs[SUBSET_DEF] >>
+      first_x_assum drule >> strip_tac >> first_x_assum drule >> strip_tac >> gvs[]
+      )
+    >- (CCONTR_TAC >> gvs[] >> first_x_assum drule >> simp[])
+    >- (CCONTR_TAC >> gvs[SUBSET_DEF] >> first_x_assum drule >> simp[])
+    >- (CCONTR_TAC >> gvs[SUBSET_DEF] >> first_x_assum drule >> simp[])
+    >- (CCONTR_TAC >> gvs[] >> first_x_assum drule >> simp[])
+    >- (CCONTR_TAC >> gvs[SUBSET_DEF] >> first_x_assum drule >> simp[])
+    >- (CCONTR_TAC >> gvs[SUBSET_DEF] >> first_x_assum drule >> simp[])
+    >- (
+      gvs[new_vars_def, BIGUNION_FRANGE_maunion, GSYM CONJ_ASSOC] >>
+      simp[new_vars_constraint_def, pure_vars] >>
+      rw[] >> rename1 `foo ⊆ _` >> gvs[SUBSET_DEF] >> rw[] >>
+      first_x_assum drule >> rw[]
+      )
+    )
+  >- ( (* Act *)
+    gvs[inferM_rws] >>
+    Cases_on `es` >> gvs[] >> Cases_on `t` >> gvs[] >> every_case_tac >> gvs[] >>
+    first_x_assum drule_all >> strip_tac >> gvs[] >>
+    goal_assum drule >> simp[Once minfer_cases, PULL_EXISTS, GSYM CONJ_ASSOC] >>
+    goal_assum $ drule_at Any >> simp[] >> rw[] >>
+    gvs[new_vars_def, new_vars_constraint_def, pure_vars]
+    )
+  >- ( (* Alloc *)
+    gvs[inferM_rws] >>
+    Cases_on `es` >> gvs[] >> Cases_on `t` >> gvs[] >>
+    Cases_on `t'` >> gvs[inferM_rws] >> every_case_tac >> gvs[] >>
+    first_x_assum drule_all >> strip_tac >> gvs[] >>
+    last_x_assum drule >> impl_tac
+    >- (rw[] >> last_x_assum drule >> simp[]) >>
+    strip_tac >> gvs[] >>
+    simp[Once minfer_cases, PULL_EXISTS] >>
+    ntac 2 $ goal_assum $ drule_at Any >> rw[]
+    >- (
+      gvs[assumptions_rel_def] >> simp[PULL_FORALL, aunion_def] >>
+      rpt gen_tac >> DEP_REWRITE_TAC[lookup_unionWith] >>
+      DEP_REWRITE_TAC[cj 1 unionWith_thm, cj 2 unionWith_thm] >> simp[] >>
+      simp[maunion_def, FLOOKUP_FMERGE] >>
+      every_case_tac >> gvs[] >> rw[] >>
+      metis_tac[wf_union, domain_union]
+      )
+    >- (
+      simp[cvars_disjoint_def, DISJOINT_ALT] >> rw[] >> CCONTR_TAC >> gvs[SUBSET_DEF] >>
+      first_x_assum drule >> strip_tac >> first_x_assum drule >> strip_tac >> gvs[]
+      )
+    >- (
+      gvs[new_vars_def, BIGUNION_FRANGE_maunion, GSYM CONJ_ASSOC] >>
+      simp[new_vars_constraint_def, pure_vars] >>
+      rw[] >> rename1 `foo ⊆ _` >> gvs[SUBSET_DEF] >> rw[] >>
+      first_x_assum drule >> rw[]
+      )
+    )
+  >- ( (* Length *)
+    gvs[inferM_rws] >>
+    Cases_on `es` >> gvs[] >> Cases_on `t` >> gvs[] >> every_case_tac >> gvs[] >>
+    first_x_assum drule_all >> strip_tac >> gvs[] >>
+    goal_assum drule >> simp[Once minfer_cases, PULL_EXISTS, GSYM CONJ_ASSOC] >>
+    goal_assum $ drule_at Any >> irule_at Any EQ_REFL >> rw[]
+    >- (CCONTR_TAC >> gvs[] >> first_x_assum drule >> simp[])
+    >- (CCONTR_TAC >> gvs[SUBSET_DEF] >> first_x_assum drule >> simp[])
+    >- (
+      gvs[new_vars_def, BIGUNION_FRANGE_maunion, GSYM CONJ_ASSOC] >>
+      simp[new_vars_constraint_def, pure_vars] >>
+      rw[] >> rename1 `foo ⊆ _` >> gvs[SUBSET_DEF] >> rw[] >>
+      first_x_assum drule >> rw[]
+      )
+    )
+  >- ( (* Deref *)
+    gvs[inferM_rws] >>
+    Cases_on `es` >> gvs[] >> Cases_on `t` >> gvs[] >>
+    Cases_on `t'` >> gvs[inferM_rws] >> every_case_tac >> gvs[] >>
+    first_x_assum drule_all >> strip_tac >> gvs[] >>
+    last_x_assum drule >> impl_tac
+    >- (rw[] >> last_x_assum drule >> simp[]) >>
+    strip_tac >> gvs[] >>
+    simp[Once minfer_cases, PULL_EXISTS] >>
+    ntac 2 $ goal_assum $ drule_at Any >> rw[]
+    >- (
+      gvs[assumptions_rel_def] >> simp[PULL_FORALL, aunion_def] >>
+      rpt gen_tac >> DEP_REWRITE_TAC[lookup_unionWith] >>
+      DEP_REWRITE_TAC[cj 1 unionWith_thm, cj 2 unionWith_thm] >> simp[] >>
+      simp[maunion_def, FLOOKUP_FMERGE] >>
+      every_case_tac >> gvs[] >> rw[] >>
+      metis_tac[wf_union, domain_union]
+      )
+    >- (rw[EXTENSION] >> eq_tac >> rw[] >> simp[])
+    >- (
+      simp[cvars_disjoint_def, DISJOINT_ALT] >> rw[] >> CCONTR_TAC >> gvs[SUBSET_DEF] >>
+      first_x_assum drule >> strip_tac >> first_x_assum drule >> strip_tac >> gvs[]
+      )
+    >- (CCONTR_TAC >> gvs[] >> first_x_assum drule >> simp[])
+    >- (CCONTR_TAC >> gvs[SUBSET_DEF] >> first_x_assum drule >> simp[])
+    >- (CCONTR_TAC >> gvs[SUBSET_DEF] >> first_x_assum drule >> simp[])
+    >- (
+      gvs[new_vars_def, BIGUNION_FRANGE_maunion, GSYM CONJ_ASSOC] >>
+      simp[new_vars_constraint_def, pure_vars] >>
+      rw[] >> rename1 `foo ⊆ _` >> gvs[SUBSET_DEF] >> rw[] >>
+      first_x_assum drule >> rw[]
+      )
+    )
+  >- ( (* Update *)
+    gvs[inferM_rws] >>
+    Cases_on `es` >> gvs[] >> Cases_on `t` >> gvs[] >>
+    Cases_on `t'` >> gvs[inferM_rws] >> every_case_tac >> gvs[] >>
+    first_x_assum drule_all >> strip_tac >> gvs[] >>
+    first_x_assum drule >> impl_tac
+    >- (rw[] >> last_x_assum drule >> simp[]) >>
+    strip_tac >> gvs[] >>
+    first_x_assum drule >> impl_tac
+    >- (rw[] >> last_x_assum drule >> simp[]) >>
+    strip_tac >> gvs[] >>
+    simp[Once minfer_cases, PULL_EXISTS, GSYM CONJ_ASSOC] >>
+    ntac 3 $ goal_assum $ drule_at Any >> simp[] >>
+    qexistsl_tac [`maunion (maunion mas' mas) mas''`,`r''`] >> rw[]
+    >- (
+      gvs[assumptions_rel_def] >> simp[PULL_FORALL, aunion_def] >>
+      rpt gen_tac >> DEP_REWRITE_TAC[lookup_unionWith] >>
+      DEP_REWRITE_TAC[cj 1 unionWith_thm, cj 2 unionWith_thm] >> simp[] >>
+      simp[maunion_def, FLOOKUP_FMERGE] >>
+      every_case_tac >> gvs[] >> rw[] >>
+      DEP_REWRITE_TAC[wf_union] >>
+      simp[domain_union, AC UNION_ASSOC UNION_COMM] >> metis_tac[]
+      )
+    >- (rw[EXTENSION] >> eq_tac >> rw[] >> simp[])
+    >- (
+      simp[cvars_disjoint_def, list_disjoint_alt_def, DISJOINT_ALT] >> rw[] >>
+      CCONTR_TAC >> gvs[SUBSET_DEF] >>
+      Cases_on `left` >> gvs[] >> Cases_on `t` >> gvs[]
+      >- (ntac 2 (first_x_assum drule >> strip_tac) >> gvs[])
+      >- (ntac 2 (first_x_assum drule >> strip_tac) >> gvs[]) >>
+      Cases_on `t'` >> gvs[] >>
+      first_x_assum drule >> strip_tac >> first_x_assum drule >> strip_tac >> gvs[]
+      )
+    >- (CCONTR_TAC >> gvs[] >> first_x_assum drule >> simp[])
+    >- (CCONTR_TAC >> gvs[SUBSET_DEF] >> first_x_assum drule >> simp[])
+    >- (CCONTR_TAC >> gvs[SUBSET_DEF] >> first_x_assum drule >> simp[])
+    >- (CCONTR_TAC >> gvs[SUBSET_DEF] >> first_x_assum drule >> simp[])
+    >- (
+      gvs[new_vars_def, BIGUNION_FRANGE_maunion, GSYM CONJ_ASSOC] >>
+      simp[new_vars_constraint_def, pure_vars] >>
+      rw[] >> rename1 `foo ⊆ _` >> gvs[SUBSET_DEF] >> rw[] >>
+      first_x_assum drule >> rw[]
+      )
+    )
+  >- ( (* True *)
+    gvs[inferM_rws] >> every_case_tac >> gvs[] >>
+    simp[Once minfer_cases, new_vars_def, pure_vars, assumptions_rel_def]
+    )
+  >- ( (* False *)
+    gvs[inferM_rws] >> every_case_tac >> gvs[] >>
+    simp[Once minfer_cases, new_vars_def, pure_vars, assumptions_rel_def]
+    )
+  >- ( (* Subscript *)
+    gvs[inferM_rws] >> every_case_tac >> gvs[] >>
+    simp[Once minfer_cases] >> irule_at Any OR_INTRO_THM1 >>
+    simp[new_vars_def, pure_vars, assumptions_rel_def]
+    )
+  >- ( (* Cons and Exception *)
+    gvs[inferM_rws] >> every_case_tac >> gvs[] >> pairarg_tac >> gvs[] >>
+    every_case_tac >> gvs[]
+    >- ( (* Exception *)
+      rename1 `_ = SOME ((_,_,cs),_)` >>
+      qsuff_tac
+        `∃ass css.
+          LIST_REL (λ(e,ty) (a,c). minfer ns (domain mset) e a c ty)
+            (ZIP (es,tys)) (ZIP (ass,css)) ∧
+          assumptions_rel as (FOLDR maunion FEMPTY ass) ∧
+          BIGUNION (set css) = set (MAP to_mconstraint cs) ∧
+          cvars_disjoint (ZIP (ass, ZIP (css, tys))) ∧
+          new_vars (FOLDR maunion FEMPTY ass)
+            (BIGUNION (set css)) (iFunctions tys Exception) ⊆ {v | n ≤ v ∧ v < m} ∧
+          LENGTH es = LENGTH tys ∧ LENGTH ass = LENGTH css ∧
+          n ≤ m`
+      >- (
+        rw[] >> gvs[] >>
+        simp[Once minfer_cases, PULL_EXISTS] >>
+        rpt $ goal_assum $ drule_at Any >>
+        simp[MAP2_MAP, MAP_MAP_o, combinTheory.o_DEF, LAMBDA_PROD] >>
+        simp[reserved_cns_def] >>
+        gvs[new_vars_def, LIST_TO_SET_MAP, IMAGE_IMAGE,
+            combinTheory.o_DEF, LAMBDA_PROD, pure_vars] >>
+        simp[BIGUNION_SUBSET, PULL_EXISTS] >>
+        gen_tac >> DEP_REWRITE_TAC[MEM_ZIP] >> simp[] >> strip_tac >> gvs[] >>
+        gvs[pure_vars_iFunctions, BIGUNION_SUBSET, MEM_MAP, PULL_EXISTS] >>
+        last_x_assum irule >> simp[EL_MEM]
+        ) >>
+      qpat_x_assum `FOLDR _ _ _ _ = _` mp_tac >>
+      ntac 3 $ pop_assum kall_tac >> pop_assum mp_tac >>
+      ntac 13 $ last_x_assum kall_tac >>
+      map_every qid_spec_tac [`m`,`n`,`tys`,`as`,`cs`] >>
+      Induct_on `es` >> rw[] >> simp[]
+      >- (
+        qexistsl_tac [`[]`,`[]`] >> simp[assumptions_rel_def, iFunctions_def] >>
+        simp[cvars_disjoint_def, new_vars_def, list_disjoint_def, pure_vars]
+        ) >>
+      every_case_tac >> gvs[PULL_EXISTS, EXISTS_PROD] >>
+      rename1 `FOLDR _ _ _ _ = SOME ((tysrest,asrest,csrest),r)` >>
+      rename1 `infer _ _ _ _ = SOME ((ty,as,cs),m)` >>
+      last_x_assum drule >> strip_tac >> gvs[] >>
+      last_x_assum $ qspec_then `h` mp_tac >> simp[] >>
+      disch_then drule >> impl_tac >- (rw[] >> first_x_assum drule >> rw[]) >>
+      strip_tac >> gvs[] >> ntac 2 $ goal_assum $ drule_at Any >>
+      once_rewrite_tac[GSYM ZIP] >> irule_at Any EQ_REFL >> simp[] >> rw[]
+      >- (
+        gvs[assumptions_rel_def, aunion_def, PULL_FORALL] >> rpt gen_tac >>
+        DEP_REWRITE_TAC[cj 1 unionWith_thm, cj 2 unionWith_thm, lookup_unionWith] >>
+        gvs[maunion_def, FLOOKUP_FMERGE] >>
+        ntac 2 $ first_x_assum $ qspecl_then [`s`,`s'`] assume_tac >>
+        every_case_tac >> gvs[] >> rw[] >>
+        metis_tac[wf_union, domain_union, UNION_COMM]
+        )
+      >- (
+        gvs[cvars_disjoint_def] >>
+        once_rewrite_tac[CONS_APPEND] >> rewrite_tac[list_disjoint_append] >>
+        simp[MEM_MAP, EXISTS_PROD, PULL_EXISTS] >> rpt gen_tac >>
+        DEP_REWRITE_TAC[MEM_ZIP] >> DEP_REWRITE_TAC[cj 1 LENGTH_ZIP] >> simp[] >>
+        imp_res_tac LIST_REL_LENGTH >> gvs[] >> simp[PULL_EXISTS] >> rw[] >>
+        pop_assum mp_tac >> DEP_REWRITE_TAC[EL_ZIP] >> simp[] >> strip_tac >> gvs[] >>
+        irule SUBSET_DISJOINT >> goal_assum $ drule_at Any >>
+        qexists_tac `{v | n ≤ v ∧ v < r}` >>
+        conj_tac >- rw[DISJOINT_ALT] >> gvs[] >>
+        irule SUBSET_TRANS >> goal_assum $ drule_at Any >>
+        gvs[new_vars_def, BIGUNION_SUBSET, pure_vars, PULL_EXISTS] >> rw[]
+        >- (
+          simp[SUBSET_DEF] >> rw[] >> disj1_tac >> disj1_tac >>
+          gvs[IN_FRANGE_FLOOKUP, FLOOKUP_FOLDR_maunion, PULL_EXISTS,
+              GSYM CONJ_ASSOC, FLOOKUP_DEF, BIGUNION_SUBSET] >>
+          rpt $ goal_assum $ drule_at Any >> simp[EL_MEM]
+          )
+        >- (
+          simp[SUBSET_DEF] >> rw[] >> disj1_tac >> disj2_tac >>
+          simp[PULL_EXISTS] >> goal_assum drule >>
+          qpat_x_assum `BIGUNION _ = _` mp_tac >> simp[EXTENSION] >>
+          disch_then $ irule o iffLR >> goal_assum drule >> simp[EL_MEM]
+          )
+        >- (
+          simp[SUBSET_DEF] >> rw[] >> disj2_tac >> simp[MEM_MAP, PULL_EXISTS] >>
+          simp[pure_vars_iFunctions, pure_vars] >>
+          simp[MEM_MAP, PULL_EXISTS] >> goal_assum drule >> simp[EL_MEM]
+          )
+        )
+      >- (
+        gvs[new_vars_def, BIGUNION_FRANGE_maunion, GSYM CONJ_ASSOC,
+            pure_vars, pure_vars_iFunctions] >> rw[] >>
+        rename1 `foo ⊆ _` >> gvs[SUBSET_DEF] >> rw[] >> first_x_assum drule >> rw[]
+        )
+      )
+    >- (
+      gvs[inferM_rws] >> rename1 `_ = SOME ((_,_,cs),m)` >>
+      qsuff_tac
+        `∃ass css.
+          LIST_REL (λ(e,ty) (a,c). minfer ns (domain mset) e a c ty)
+            (ZIP (es,tys)) (ZIP (ass,css)) ∧
+          assumptions_rel as (FOLDR maunion FEMPTY ass) ∧
+          BIGUNION (set css) = set (MAP to_mconstraint cs) ∧
+          cvars_disjoint (ZIP (ass, ZIP (css, tys))) ∧
+          new_vars (FOLDR maunion FEMPTY ass)
+            (BIGUNION (set css)) (iFunctions tys Exception) ⊆ {v | n ≤ v ∧ v < m} ∧
+          LENGTH es = LENGTH tys ∧ LENGTH ass = LENGTH css ∧
+          n ≤ m`
+      >- (
+        rw[] >> gvs[] >>
+        drule infer_cons_SOME >>
+        disch_then $ qspec_then `FST ns` assume_tac >> gvs[] >>
+        rename [`ALOOKUP _ _ = SOME schemes`,`oEL tyid _ = SOME (arity,_)`] >>
+        simp[Once minfer_cases, PULL_EXISTS] >>
+        rpt $ goal_assum $ drule_at Any >> simp[] >> irule_at Any EQ_REFL >>
+        DEP_REWRITE_TAC[MAP2_MAP] >> gvs[oEL_THM] >>
+        simp[MAP2_MAP, MAP_MAP_o, combinTheory.o_DEF, LAMBDA_PROD] >>
+        simp[reserved_cns_def] >> conj_tac
+        >- (
+          drule LIST_REL_LENGTH >>
+          DEP_REWRITE_TAC[cj 1 LENGTH_ZIP] >> simp[] >> rw[] >> gvs[] >>
+          simp[EVERY_GENLIST, EVERY_MEM, FORALL_PROD] >> rw[]
+          >- (CCONTR_TAC >> gvs[] >> first_x_assum drule >> simp[]) >>
+          pop_assum mp_tac >> DEP_REWRITE_TAC[MEM_ZIP] >> simp[MIN_DEF] >>
+          strip_tac >> gvs[] >>
+          pop_assum mp_tac >> DEP_REWRITE_TAC[EL_ZIP] >> simp[] >>
+          strip_tac >> gvs[] >>
+          qsuff_tac
+            `new_vars (EL n'' ass) (EL n'' css) (EL n'' tys) ⊆ {v | n ≤ v ∧ v < m}`
+          >- (rw[SUBSET_DEF] >> CCONTR_TAC >> gvs[] >> first_x_assum drule >> simp[]) >>
+          irule SUBSET_TRANS >> goal_assum $ drule_at Any >>
+          gvs[new_vars_def, BIGUNION_SUBSET, pure_vars, PULL_EXISTS] >> rw[]
+          >- (
+            simp[SUBSET_DEF] >> rw[] >> disj1_tac >> disj1_tac >>
+            gvs[IN_FRANGE_FLOOKUP, FLOOKUP_FOLDR_maunion, PULL_EXISTS,
+                GSYM CONJ_ASSOC, FLOOKUP_DEF, BIGUNION_SUBSET] >>
+            rpt $ goal_assum $ drule_at Any >> simp[EL_MEM]
+            )
+          >- (
+            simp[SUBSET_DEF] >> rw[] >> disj1_tac >> disj2_tac >>
+            simp[PULL_EXISTS] >> goal_assum drule >>
+            qpat_x_assum `BIGUNION _ = _` mp_tac >> simp[EXTENSION] >>
+            disch_then $ irule o iffLR >> goal_assum drule >> simp[EL_MEM]
+            )
+          >- (
+            simp[SUBSET_DEF] >> rw[] >> disj2_tac >> simp[MEM_MAP, PULL_EXISTS] >>
+            simp[pure_vars_iFunctions, pure_vars] >>
+            simp[MEM_MAP, PULL_EXISTS] >> goal_assum drule >> simp[EL_MEM]
+            )
+          )
+        >- (
+          gvs[new_vars_def, BIGUNION_SUBSET, pure_vars, pure_vars_iFunctions,
+              PULL_EXISTS, IN_FRANGE_FLOOKUP, FLOOKUP_FOLDR_maunion, GSYM CONJ_ASSOC,
+              MEM_MAP, EXISTS_PROD, MEM_GENLIST, FLOOKUP_DEF, MEM_ZIP] >> rw[]
+          >- (
+            first_x_assum drule_all >> rw[SUBSET_DEF] >>
+            first_x_assum drule >> simp[]
+            )
+          >- (
+            last_x_assum $ qspec_then `EL n' tys` mp_tac >> simp[EL_MEM] >>
+            rw[SUBSET_DEF] >> first_x_assum drule >> simp[]
+            )
+          >- (
+            irule SUBSET_TRANS >> irule_at Any pure_vars_isubst_SUBSET >>
+            simp[BIGUNION_SUBSET, MAP_MAP_o, combinTheory.o_DEF, pure_vars] >>
+            simp[MEM_MAP, MEM_GENLIST, PULL_EXISTS]
+            )
+          >- (
+            first_x_assum drule >> rw[SUBSET_DEF] >> first_x_assum drule >> simp[]
+            )
+          )
+        ) >>
+      qpat_x_assum `FOLDR _ _ _ _ = _` mp_tac >>
+      ntac 3 $ pop_assum kall_tac >> pop_assum mp_tac >>
+      ntac 13 $ last_x_assum kall_tac >>
+      map_every qid_spec_tac [`m`,`n`,`tys`,`as`,`cs`] >>
+      Induct_on `es` >> rw[] >> simp[]
+      >- (
+        qexistsl_tac [`[]`,`[]`] >> simp[assumptions_rel_def, iFunctions_def] >>
+        simp[cvars_disjoint_def, new_vars_def, list_disjoint_def, pure_vars]
+        ) >>
+      every_case_tac >> gvs[PULL_EXISTS, EXISTS_PROD] >>
+      rename1 `FOLDR _ _ _ _ = SOME ((tysrest,asrest,csrest),r)` >>
+      rename1 `infer _ _ _ _ = SOME ((ty,as,cs),m)` >>
+      last_x_assum drule >> strip_tac >> gvs[] >>
+      last_x_assum $ qspec_then `h` mp_tac >> simp[] >>
+      disch_then drule >> impl_tac >- (rw[] >> first_x_assum drule >> rw[]) >>
+      strip_tac >> gvs[] >> ntac 2 $ goal_assum $ drule_at Any >>
+      once_rewrite_tac[GSYM ZIP] >> irule_at Any EQ_REFL >> simp[] >> rw[]
+      >- (
+        gvs[assumptions_rel_def, aunion_def, PULL_FORALL] >> rpt gen_tac >>
+        DEP_REWRITE_TAC[cj 1 unionWith_thm, cj 2 unionWith_thm, lookup_unionWith] >>
+        gvs[maunion_def, FLOOKUP_FMERGE] >>
+        ntac 2 $ first_x_assum $ qspecl_then [`s`,`s'`] assume_tac >>
+        every_case_tac >> gvs[] >> rw[] >>
+        metis_tac[wf_union, domain_union, UNION_COMM]
+        )
+      >- (
+        gvs[cvars_disjoint_def] >>
+        once_rewrite_tac[CONS_APPEND] >> rewrite_tac[list_disjoint_append] >>
+        simp[MEM_MAP, EXISTS_PROD, PULL_EXISTS] >> rpt gen_tac >>
+        DEP_REWRITE_TAC[MEM_ZIP] >> DEP_REWRITE_TAC[cj 1 LENGTH_ZIP] >> simp[] >>
+        imp_res_tac LIST_REL_LENGTH >> gvs[] >> simp[PULL_EXISTS] >> rw[] >>
+        pop_assum mp_tac >> DEP_REWRITE_TAC[EL_ZIP] >> simp[] >> strip_tac >> gvs[] >>
+        irule SUBSET_DISJOINT >> goal_assum $ drule_at Any >>
+        qexists_tac `{v | n ≤ v ∧ v < r}` >>
+        conj_tac >- rw[DISJOINT_ALT] >> gvs[] >>
+        irule SUBSET_TRANS >> goal_assum $ drule_at Any >>
+        gvs[new_vars_def, BIGUNION_SUBSET, pure_vars, PULL_EXISTS] >> rw[]
+        >- (
+          simp[SUBSET_DEF] >> rw[] >> disj1_tac >> disj1_tac >>
+          gvs[IN_FRANGE_FLOOKUP, FLOOKUP_FOLDR_maunion, PULL_EXISTS,
+              GSYM CONJ_ASSOC, FLOOKUP_DEF, BIGUNION_SUBSET] >>
+          rpt $ goal_assum $ drule_at Any >> simp[EL_MEM]
+          )
+        >- (
+          simp[SUBSET_DEF] >> rw[] >> disj1_tac >> disj2_tac >>
+          simp[PULL_EXISTS] >> goal_assum drule >>
+          qpat_x_assum `BIGUNION _ = _` mp_tac >> simp[EXTENSION] >>
+          disch_then $ irule o iffLR >> goal_assum drule >> simp[EL_MEM]
+          )
+        >- (
+          simp[SUBSET_DEF] >> rw[] >> disj2_tac >> simp[MEM_MAP, PULL_EXISTS] >>
+          simp[pure_vars_iFunctions, pure_vars] >>
+          simp[MEM_MAP, PULL_EXISTS] >> goal_assum drule >> simp[EL_MEM]
+          )
+        )
+      >- (
+        gvs[new_vars_def, BIGUNION_FRANGE_maunion, GSYM CONJ_ASSOC,
+            pure_vars, pure_vars_iFunctions] >> rw[] >>
+        rename1 `foo ⊆ _` >> gvs[SUBSET_DEF] >> rw[] >> first_x_assum drule >> rw[]
+        )
+      )
+    >- (
+      gvs[inferM_rws] >> rename1 `_ = SOME ((_,_,cs),m)` >>
+      qsuff_tac
+        `∃ass css.
+          LIST_REL (λ(e,ty) (a,c). minfer ns (domain mset) e a c ty)
+            (ZIP (es,tys)) (ZIP (ass,css)) ∧
+          assumptions_rel as (FOLDR maunion FEMPTY ass) ∧
+          BIGUNION (set css) = set (MAP to_mconstraint cs) ∧
+          cvars_disjoint (ZIP (ass, ZIP (css, tys))) ∧
+          new_vars (FOLDR maunion FEMPTY ass)
+            (BIGUNION (set css)) (iFunctions tys Exception) ⊆ {v | n ≤ v ∧ v < m} ∧
+          LENGTH es = LENGTH tys ∧ LENGTH ass = LENGTH css ∧
+          n ≤ m`
+      >- (
+        rw[] >> gvs[] >>
+        drule infer_cons_SOME >>
+        disch_then $ qspec_then `FST ns` assume_tac >> gvs[] >>
+        rename [`ALOOKUP _ _ = SOME schemes`,`oEL tyid _ = SOME (arity,_)`] >>
+        simp[Once minfer_cases, PULL_EXISTS] >>
+        rpt $ goal_assum $ drule_at Any >> simp[] >>
+        DEP_REWRITE_TAC[MAP2_MAP] >> gvs[oEL_THM] >>
+        simp[MAP2_MAP, MAP_MAP_o, combinTheory.o_DEF, LAMBDA_PROD] >>
+        simp[reserved_cns_def] >>
+        gvs[new_vars_def, pure_vars, LIST_TO_SET_MAP, IMAGE_IMAGE,
+            combinTheory.o_DEF, BIGUNION_SUBSET, PULL_EXISTS, FORALL_PROD,
+            MEM_ZIP, pure_vars_iFunctions] >>
+        rw[] >> last_x_assum irule >> simp[EL_MEM]
+        ) >>
+      qpat_x_assum `FOLDR _ _ _ _ = _` mp_tac >>
+      ntac 3 $ pop_assum kall_tac >> pop_assum mp_tac >>
+      ntac 13 $ last_x_assum kall_tac >>
+      rename1 `FOLDR _ _ _ _ = SOME (_,m)` >>
+      map_every qid_spec_tac [`m`,`n`,`tys`,`as`,`cs`] >>
+      Induct_on `es` >> rw[] >> simp[]
+      >- (
+        qexistsl_tac [`[]`,`[]`] >> simp[assumptions_rel_def, iFunctions_def] >>
+        simp[cvars_disjoint_def, new_vars_def, list_disjoint_def, pure_vars]
+        ) >>
+      every_case_tac >> gvs[PULL_EXISTS, EXISTS_PROD] >>
+      rename1 `FOLDR _ _ _ _ = SOME ((tysrest,asrest,csrest),r)` >>
+      rename1 `infer _ _ _ _ = SOME ((ty,as,cs),m)` >>
+      last_x_assum drule >> strip_tac >> gvs[] >>
+      last_x_assum $ qspec_then `h` mp_tac >> simp[] >>
+      disch_then drule >> impl_tac >- (rw[] >> first_x_assum drule >> rw[]) >>
+      strip_tac >> gvs[] >> ntac 2 $ goal_assum $ drule_at Any >>
+      once_rewrite_tac[GSYM ZIP] >> irule_at Any EQ_REFL >> simp[] >> rw[]
+      >- (
+        gvs[assumptions_rel_def, aunion_def, PULL_FORALL] >> rpt gen_tac >>
+        DEP_REWRITE_TAC[cj 1 unionWith_thm, cj 2 unionWith_thm, lookup_unionWith] >>
+        gvs[maunion_def, FLOOKUP_FMERGE] >>
+        ntac 2 $ first_x_assum $ qspecl_then [`s`,`s'`] assume_tac >>
+        every_case_tac >> gvs[] >> rw[] >>
+        metis_tac[wf_union, domain_union, UNION_COMM]
+        )
+      >- (
+        gvs[cvars_disjoint_def] >>
+        once_rewrite_tac[CONS_APPEND] >> rewrite_tac[list_disjoint_append] >>
+        simp[MEM_MAP, EXISTS_PROD, PULL_EXISTS] >> rpt gen_tac >>
+        DEP_REWRITE_TAC[MEM_ZIP] >> DEP_REWRITE_TAC[cj 1 LENGTH_ZIP] >> simp[] >>
+        imp_res_tac LIST_REL_LENGTH >> gvs[] >> simp[PULL_EXISTS] >> rw[] >>
+        pop_assum mp_tac >> DEP_REWRITE_TAC[EL_ZIP] >> simp[] >> strip_tac >> gvs[] >>
+        irule SUBSET_DISJOINT >> goal_assum $ drule_at Any >>
+        qexists_tac `{v | n ≤ v ∧ v < r}` >>
+        conj_tac >- rw[DISJOINT_ALT] >> gvs[] >>
+        irule SUBSET_TRANS >> goal_assum $ drule_at Any >>
+        gvs[new_vars_def, BIGUNION_SUBSET, pure_vars, PULL_EXISTS] >> rw[]
+        >- (
+          simp[SUBSET_DEF] >> rw[] >> disj1_tac >> disj1_tac >>
+          gvs[IN_FRANGE_FLOOKUP, FLOOKUP_FOLDR_maunion, PULL_EXISTS,
+              GSYM CONJ_ASSOC, FLOOKUP_DEF, BIGUNION_SUBSET] >>
+          rpt $ goal_assum $ drule_at Any >> simp[EL_MEM]
+          )
+        >- (
+          simp[SUBSET_DEF] >> rw[] >> disj1_tac >> disj2_tac >>
+          simp[PULL_EXISTS] >> goal_assum drule >>
+          qpat_x_assum `BIGUNION _ = _` mp_tac >> simp[EXTENSION] >>
+          disch_then $ irule o iffLR >> goal_assum drule >> simp[EL_MEM]
+          )
+        >- (
+          simp[SUBSET_DEF] >> rw[] >> disj2_tac >> simp[MEM_MAP, PULL_EXISTS] >>
+          simp[pure_vars_iFunctions, pure_vars] >>
+          simp[MEM_MAP, PULL_EXISTS] >> goal_assum drule >> simp[EL_MEM]
+          )
+        )
+      >- (
+        gvs[new_vars_def, BIGUNION_FRANGE_maunion, GSYM CONJ_ASSOC,
+            pure_vars, pure_vars_iFunctions] >> rw[] >>
+        rename1 `foo ⊆ _` >> gvs[SUBSET_DEF] >> rw[] >> first_x_assum drule >> rw[]
+        )
+      )
+    )
+  >- ( (* AtomOp *)
+    Cases_on `infer_atom_op (LENGTH es) aop` >> gvs[inferM_rws] >>
+    pairarg_tac >> gvs[] >>
+    every_case_tac >> gvs[] >> rename1 `FOLDR _ _ _ _ = SOME ((tys,as,cs),m)` >>
+    qsuff_tac
+      `∃ass css.
+        LIST_REL (λ(e,ty) (a,c). minfer ns (domain mset) e a c ty)
+          (ZIP (es,tys)) (ZIP (ass,css)) ∧
+        assumptions_rel as (FOLDR maunion FEMPTY ass) ∧
+        BIGUNION (set css) = set (MAP to_mconstraint cs) ∧
+        cvars_disjoint (ZIP (ass, ZIP (css, tys))) ∧
+        new_vars (FOLDR maunion FEMPTY ass)
+          (BIGUNION (set css)) (iFunctions tys Exception) ⊆ {v | n ≤ v ∧ v < m} ∧
+        LENGTH es = LENGTH tys ∧ LENGTH ass = LENGTH css ∧
+        n ≤ m`
+    >- (
+      rw[] >> gvs[] >>
+      simp[Once minfer_cases, PULL_EXISTS] >>
+      rpt $ goal_assum $ drule_at Any >> simp[] >>
+      DEP_REWRITE_TAC[MAP2_MAP] >> gvs[oEL_THM] >>
+      simp[MAP2_MAP, MAP_MAP_o, combinTheory.o_DEF, LAMBDA_PROD] >>
+      imp_res_tac infer_atom_op_LENGTH >> gvs[] >>
+      gvs[new_vars_def, LIST_TO_SET_MAP, IMAGE_IMAGE, combinTheory.o_DEF,
+          BIGUNION_SUBSET, PULL_EXISTS, MEM_ZIP, pure_vars, pure_vars_iFunctions] >>
+      rw[] >> last_x_assum irule >> simp[EL_MEM]
+      ) >>
+    qpat_x_assum `FOLDR _ _ _ _ = _` mp_tac >>
+    pop_assum kall_tac >> pop_assum mp_tac >> last_x_assum mp_tac >>
+    map_every qid_spec_tac [`m`,`n`,`tys`,`as`,`cs`] >>
+    Induct_on `es` >> rw[] >> simp[]
+    >- (
+      qexistsl_tac [`[]`,`[]`] >> simp[assumptions_rel_def, iFunctions_def] >>
+      simp[cvars_disjoint_def, new_vars_def, list_disjoint_def, pure_vars]
+      ) >>
+    every_case_tac >> gvs[PULL_EXISTS, EXISTS_PROD] >>
+    rename1 `FOLDR _ _ _ _ = SOME ((tysrest,asrest,csrest),r)` >>
+    rename1 `infer _ _ _ _ = SOME ((ty,as,cs),m)` >>
+    last_x_assum drule >> strip_tac >> gvs[] >>
+    last_x_assum $ qspec_then `h` mp_tac >> simp[] >>
+    disch_then drule >> impl_tac >- (rw[] >> first_x_assum drule >> rw[]) >>
+    strip_tac >> gvs[] >> ntac 2 $ goal_assum $ drule_at Any >>
+    once_rewrite_tac[GSYM ZIP] >> irule_at Any EQ_REFL >> simp[] >> rw[]
+    >- (
+      gvs[assumptions_rel_def, aunion_def, PULL_FORALL] >> rpt gen_tac >>
+      DEP_REWRITE_TAC[cj 1 unionWith_thm, cj 2 unionWith_thm, lookup_unionWith] >>
+      gvs[maunion_def, FLOOKUP_FMERGE] >>
+      ntac 2 $ first_x_assum $ qspecl_then [`s`,`s'`] assume_tac >>
+      every_case_tac >> gvs[] >> rw[] >>
+      metis_tac[wf_union, domain_union, UNION_COMM]
+      )
+    >- (
+      gvs[cvars_disjoint_def] >>
+      once_rewrite_tac[CONS_APPEND] >> rewrite_tac[list_disjoint_append] >>
+      simp[MEM_MAP, EXISTS_PROD, PULL_EXISTS] >> rpt gen_tac >>
+      DEP_REWRITE_TAC[MEM_ZIP] >> DEP_REWRITE_TAC[cj 1 LENGTH_ZIP] >> simp[] >>
+      imp_res_tac LIST_REL_LENGTH >> gvs[] >> simp[PULL_EXISTS] >> rw[] >>
+      pop_assum mp_tac >> DEP_REWRITE_TAC[EL_ZIP] >> simp[] >> strip_tac >> gvs[] >>
+      irule SUBSET_DISJOINT >> goal_assum $ drule_at Any >>
+      qexists_tac `{v | n ≤ v ∧ v < r}` >>
+      conj_tac >- rw[DISJOINT_ALT] >> gvs[] >>
+      irule SUBSET_TRANS >> goal_assum $ drule_at Any >>
+      gvs[new_vars_def, BIGUNION_SUBSET, pure_vars, PULL_EXISTS] >> rw[]
+      >- (
+        simp[SUBSET_DEF] >> rw[] >> disj1_tac >> disj1_tac >>
+        gvs[IN_FRANGE_FLOOKUP, FLOOKUP_FOLDR_maunion, PULL_EXISTS,
+            GSYM CONJ_ASSOC, FLOOKUP_DEF, BIGUNION_SUBSET] >>
+        rpt $ goal_assum $ drule_at Any >> simp[EL_MEM]
+        )
+      >- (
+        simp[SUBSET_DEF] >> rw[] >> disj1_tac >> disj2_tac >>
+        simp[PULL_EXISTS] >> goal_assum drule >>
+        qpat_x_assum `BIGUNION _ = _` mp_tac >> simp[EXTENSION] >>
+        disch_then $ irule o iffLR >> goal_assum drule >> simp[EL_MEM]
+        )
+      >- (
+        simp[SUBSET_DEF] >> rw[] >> disj2_tac >> simp[MEM_MAP, PULL_EXISTS] >>
+        simp[pure_vars_iFunctions, pure_vars] >>
+        simp[MEM_MAP, PULL_EXISTS] >> goal_assum drule >> simp[EL_MEM]
+        )
+      )
+    >- (
+      gvs[new_vars_def, BIGUNION_FRANGE_maunion, GSYM CONJ_ASSOC,
+          pure_vars, pure_vars_iFunctions] >> rw[] >>
+      rename1 `foo ⊆ _` >> gvs[SUBSET_DEF] >> rw[] >> first_x_assum drule >> rw[]
+      )
+    )
+  >- ( (* Seq *)
+    gvs[inferM_rws] >> every_case_tac >> gvs[] >>
+    pairarg_tac >> gvs[] >> every_case_tac >> gvs[] >>
+    first_x_assum drule_all >> strip_tac >> gvs[] >>
+    last_x_assum drule >> impl_tac
+    >- (rw[] >> last_x_assum drule >> simp[]) >>
+    strip_tac >> gvs[] >>
+    simp[Once minfer_cases, PULL_EXISTS] >>
+    ntac 2 $ goal_assum $ drule_at Any >> rw[]
+    >- (
+      gvs[assumptions_rel_def] >> simp[PULL_FORALL, aunion_def] >>
+      rpt gen_tac >> DEP_REWRITE_TAC[lookup_unionWith] >>
+      DEP_REWRITE_TAC[cj 1 unionWith_thm, cj 2 unionWith_thm] >> simp[] >>
+      simp[maunion_def, FLOOKUP_FMERGE] >>
+      every_case_tac >> gvs[] >> rw[] >>
+      metis_tac[wf_union, domain_union]
+      )
+    >- (
+      simp[cvars_disjoint_def, DISJOINT_ALT] >> rw[] >> CCONTR_TAC >> gvs[SUBSET_DEF] >>
+      first_x_assum drule >> strip_tac >> first_x_assum drule >> strip_tac >> gvs[]
+      )
+    >- (
+      gvs[new_vars_def, BIGUNION_FRANGE_maunion, GSYM CONJ_ASSOC] >>
+      simp[new_vars_constraint_def, pure_vars] >>
+      rw[] >> rename1 `foo ⊆ _` >> gvs[SUBSET_DEF] >> rw[] >>
+      first_x_assum drule >> rw[]
+      )
+    )
+  >- gvs[fail_def] (* App empty case *)
+  >- ( (* App non-empty case *)
+    gvs[inferM_rws] >> every_case_tac >> gvs[] >>
+    pairarg_tac >> gvs[] >> every_case_tac >> gvs[] >>
+    rename [
+      `FOLDR _ _ _ _ = SOME ((tys,as,cs),m)`,
+      `infer _ _ _ _ = SOME ((ety,eas,ecs),l)`] >>
+    qsuff_tac
+      `∃ass css.
+        LIST_REL (λ(e,ty) (a,c). minfer ns (domain mset) e a c ty)
+          (ZIP (es,tys)) (ZIP (ass,css)) ∧
+        assumptions_rel as (FOLDR maunion FEMPTY ass) ∧
+        BIGUNION (set css) = set (MAP to_mconstraint cs) ∧
+        cvars_disjoint (ZIP (ass, ZIP (css, tys))) ∧
+        new_vars (FOLDR maunion FEMPTY ass)
+          (BIGUNION (set css)) (iFunctions tys Exception) ⊆ {v | n ≤ v ∧ v < m} ∧
+        LENGTH es = LENGTH tys ∧ LENGTH ass = LENGTH css ∧
+        n ≤ m`
+    >- (
+      rw[] >> gvs[] >>
+      first_x_assum drule >> impl_tac >- (rw[] >> first_x_assum drule >> rw[]) >>
+      strip_tac >> gvs[] >>
+      simp[Once minfer_cases, PULL_EXISTS] >>
+      rpt $ goal_assum $ drule_at Any >> simp[] >>
+      gvs[new_vars_def, LIST_TO_SET_MAP, IMAGE_IMAGE, combinTheory.o_DEF,
+          BIGUNION_SUBSET, PULL_EXISTS, MEM_ZIP, pure_vars, pure_vars_iFunctions] >>
+      rw[]
+      >- (
+        once_rewrite_tac[maunion_comm] >>
+        gvs[assumptions_rel_def, aunion_def] >>
+        simp[PULL_FORALL] >> rpt gen_tac >>
+        DEP_REWRITE_TAC[lookup_unionWith] >>
+        DEP_REWRITE_TAC[cj 1 unionWith_thm, cj 2 unionWith_thm] >> simp[] >>
+        gvs[maunion_def, FLOOKUP_FMERGE, IN_FRANGE_FLOOKUP] >>
+        every_case_tac >> gvs[] >> rw[] >> metis_tac[wf_union, domain_union]
+        )
+      >- (
+        gvs[cvars_disjoint_def] >>
+        once_rewrite_tac[CONS_APPEND] >> rewrite_tac[list_disjoint_append] >>
+        simp[MEM_MAP, EXISTS_PROD, PULL_EXISTS] >> rpt gen_tac >>
+        DEP_REWRITE_TAC[MEM_ZIP] >> DEP_REWRITE_TAC[cj 1 LENGTH_ZIP] >> simp[] >>
+        imp_res_tac LIST_REL_LENGTH >> gvs[] >> simp[PULL_EXISTS] >> rw[] >>
+        pop_assum mp_tac >> DEP_REWRITE_TAC[EL_ZIP] >> simp[] >> strip_tac >> gvs[] >>
+        irule SUBSET_DISJOINT >>
+        qexistsl_tac [`{v | m ≤ v ∧ v < l}`,`{v | n ≤ v ∧ v < m}`] >>
+        conj_tac >- rw[DISJOINT_ALT] >> gvs[] >>
+        simp[new_vars_def, BIGUNION_SUBSET, IMAGE_IMAGE, PULL_EXISTS] >> rw[]
+        >- (
+          gvs[IN_FRANGE_FLOOKUP, FLOOKUP_FOLDR_maunion, PULL_EXISTS,
+              FLOOKUP_DEF, BIGUNION_SUBSET] >>
+          first_x_assum irule >> simp[EL_MEM] >>
+          goal_assum $ drule_at Any >> simp[EL_MEM]
+          )
+        >- (
+          qpat_x_assum `BIGUNION _ = _` mp_tac >> simp[EXTENSION] >>
+          disch_then $ mp_tac o iffLR >> simp[PULL_EXISTS] >>
+          disch_then drule >> simp[EL_MEM] >> strip_tac >> gvs[]
+          )
+        >- (last_x_assum irule >> simp[EL_MEM])
+        )
+      >- (CCONTR_TAC >> gvs[] >> first_x_assum drule >> rw[])
+      >- (
+        rw[Once DISJ_COMM] >> rw[DISJ_EQ_IMP] >>
+        first_x_assum drule >> rw[SUBSET_DEF] >>
+        CCONTR_TAC >> gvs[] >> first_x_assum drule >> rw[]
+        )
+      >- (
+        rw[Once DISJ_COMM] >> rw[DISJ_EQ_IMP] >>
+        first_x_assum drule >> rw[SUBSET_DEF] >>
+        CCONTR_TAC >> gvs[] >> first_x_assum drule >> rw[]
+        )
+      >- (CCONTR_TAC >> gvs[SUBSET_DEF] >> first_x_assum drule >> rw[])
+      >- (
+        simp[EVERY_MEM] >> gen_tac >>
+        DEP_REWRITE_TAC[MEM_ZIP] >> simp[LENGTH_ZIP] >>
+        drule LIST_REL_LENGTH >> simp[] >> rw[] >>
+        DEP_REWRITE_TAC[EL_ZIP] >> simp[] >>
+        simp[Once DISJ_COMM] >> rw[DISJ_EQ_IMP]
+        >- (
+          gvs[IN_FRANGE_FLOOKUP, FLOOKUP_FOLDR_maunion, PULL_EXISTS,
+              BIGUNION_SUBSET, FLOOKUP_DEF] >>
+          first_x_assum $ drule_at Any >> simp[EL_MEM] >>
+          disch_then $ drule_at Any >> simp[EL_MEM] >>
+          rw[SUBSET_DEF] >> CCONTR_TAC >> gvs[] >> first_x_assum drule >> simp[]
+          )
+        >- (
+          qpat_x_assum `BIGUNION _ = _` mp_tac >> simp[EXTENSION] >>
+          disch_then $ mp_tac o iffLR >> simp[PULL_EXISTS] >>
+          strip_tac >> CCONTR_TAC >> gvs[] >>
+          first_x_assum drule >> simp[EL_MEM] >> rw[] >>
+          CCONTR_TAC >> gvs[] >> last_x_assum drule >> simp[SUBSET_DEF] >>
+          goal_assum drule >> simp[]
+          )
+        >- (
+          last_x_assum $ qspec_then `EL n' tys` mp_tac >> rw[EL_MEM, SUBSET_DEF] >>
+          CCONTR_TAC >> gvs[SUBSET_DEF] >> first_x_assum drule >> simp[]
+          )
+        )
+      >- (
+        gvs[IN_FRANGE_FLOOKUP, PULL_EXISTS] >>
+        pop_assum mp_tac >> simp[Once maunion_def, FLOOKUP_FMERGE] >>
+        every_case_tac >> gvs[] >> rw[]
+        >- (
+          first_x_assum drule >> rw[SUBSET_DEF] >>
+          first_x_assum drule >> simp[]
+          )
+        >- (
+          first_x_assum drule >> rw[SUBSET_DEF] >>
+          first_x_assum drule >> simp[]
+          )
+        >- (
+          first_x_assum drule >> first_x_assum drule >>
+          rw[SUBSET_DEF] >> first_x_assum drule >> simp[]
+          )
+        )
+      >- (gvs[SUBSET_DEF] >> rw[] >> first_x_assum drule >> simp[])
+      >- (last_x_assum drule >> rw[SUBSET_DEF] >> first_x_assum drule >> simp[])
+      >- (first_x_assum drule >> rw[SUBSET_DEF] >> first_x_assum drule >> simp[])
+      >- (first_x_assum drule >> rw[SUBSET_DEF] >> first_x_assum drule >> simp[])
+      ) >>
+    qpat_x_assum `FOLDR _ _ _ _ = _` mp_tac >>
+    pop_assum kall_tac >> pop_assum mp_tac >> last_x_assum kall_tac >>
+    last_x_assum mp_tac >> last_x_assum kall_tac >>
+    map_every qid_spec_tac [`m`,`n`,`tys`,`as`,`cs`] >>
+    Induct_on `es` >> rw[] >> simp[]
+    >- (
+      qexistsl_tac [`[]`,`[]`] >> simp[assumptions_rel_def, iFunctions_def] >>
+      simp[cvars_disjoint_def, new_vars_def, list_disjoint_def, pure_vars]
+      ) >>
+    every_case_tac >> gvs[PULL_EXISTS, EXISTS_PROD] >>
+    rename1 `FOLDR _ _ _ _ = SOME ((tysrest,asrest,csrest),r)` >>
+    rename1 `infer _ _ _ _ = SOME ((ty,as,cs),m)` >>
+    last_x_assum drule >> strip_tac >> gvs[] >>
+    last_x_assum $ qspec_then `h` mp_tac >> simp[] >>
+    disch_then drule >> impl_tac >- (rw[] >> first_x_assum drule >> rw[]) >>
+    strip_tac >> gvs[] >> ntac 2 $ goal_assum $ drule_at Any >>
+    once_rewrite_tac[GSYM ZIP] >> irule_at Any EQ_REFL >> simp[] >> rw[]
+    >- (
+      gvs[assumptions_rel_def, aunion_def, PULL_FORALL] >> rpt gen_tac >>
+      DEP_REWRITE_TAC[cj 1 unionWith_thm, cj 2 unionWith_thm, lookup_unionWith] >>
+      gvs[maunion_def, FLOOKUP_FMERGE] >>
+      ntac 2 $ first_x_assum $ qspecl_then [`s`,`s'`] assume_tac >>
+      every_case_tac >> gvs[] >> rw[] >>
+      metis_tac[wf_union, domain_union, UNION_COMM]
+      )
+    >- (
+      gvs[cvars_disjoint_def] >>
+      once_rewrite_tac[CONS_APPEND] >> rewrite_tac[list_disjoint_append] >>
+      simp[MEM_MAP, EXISTS_PROD, PULL_EXISTS] >> rpt gen_tac >>
+      DEP_REWRITE_TAC[MEM_ZIP] >> DEP_REWRITE_TAC[cj 1 LENGTH_ZIP] >> simp[] >>
+      imp_res_tac LIST_REL_LENGTH >> gvs[] >> simp[PULL_EXISTS] >> rw[] >>
+      pop_assum mp_tac >> DEP_REWRITE_TAC[EL_ZIP] >> simp[] >> strip_tac >> gvs[] >>
+      irule SUBSET_DISJOINT >> goal_assum $ drule_at Any >>
+      qexists_tac `{v | n ≤ v ∧ v < r}` >>
+      conj_tac >- rw[DISJOINT_ALT] >> gvs[] >>
+      irule SUBSET_TRANS >> goal_assum $ drule_at Any >>
+      gvs[new_vars_def, BIGUNION_SUBSET, pure_vars, PULL_EXISTS] >> rw[]
+      >- (
+        simp[SUBSET_DEF] >> rw[] >> disj1_tac >> disj1_tac >>
+        gvs[IN_FRANGE_FLOOKUP, FLOOKUP_FOLDR_maunion, PULL_EXISTS,
+            GSYM CONJ_ASSOC, FLOOKUP_DEF, BIGUNION_SUBSET] >>
+        rpt $ goal_assum $ drule_at Any >> simp[EL_MEM]
+        )
+      >- (
+        simp[SUBSET_DEF] >> rw[] >> disj1_tac >> disj2_tac >>
+        simp[PULL_EXISTS] >> goal_assum drule >>
+        qpat_x_assum `BIGUNION _ = _` mp_tac >> simp[EXTENSION] >>
+        disch_then $ irule o iffLR >> goal_assum drule >> simp[EL_MEM]
+        )
+      >- (
+        simp[SUBSET_DEF] >> rw[] >> disj2_tac >> simp[MEM_MAP, PULL_EXISTS] >>
+        simp[pure_vars_iFunctions, pure_vars] >>
+        simp[MEM_MAP, PULL_EXISTS] >> goal_assum drule >> simp[EL_MEM]
+        )
+      )
+    >- (
+      gvs[new_vars_def, BIGUNION_FRANGE_maunion, GSYM CONJ_ASSOC,
+          pure_vars, pure_vars_iFunctions] >> rw[] >>
+      rename1 `foo ⊆ _` >> gvs[SUBSET_DEF] >> rw[] >> first_x_assum drule >> rw[]
+      )
+    )
+  >- gvs[fail_def] (* Lam empty case *)
+  >- ( (* Lam non-empty case *)
+    gvs[inferM_rws] >> every_case_tac >> gvs[] >>
+    pairarg_tac >> gvs[] >>
+    qpat_abbrev_tac `gens = GENLIST _ _` >>
+    last_x_assum drule >> simp[domain_list_insert] >> impl_tac
+    >- (
+      reverse $ rw[] >- (last_x_assum drule >> simp[]) >>
+      unabbrev_all_tac >> gvs[MEM_GENLIST]
+      ) >>
+    strip_tac >> gvs[] >> qexists_tac `FDIFF mas (set xs)` >> rw[]
+    >- (
+      gvs[assumptions_rel_def, PULL_FORALL] >> rpt gen_tac >>
+      DEP_REWRITE_TAC[cj 1 map_ok_list_delete, cj 2 map_ok_list_delete] >>
+      DEP_REWRITE_TAC[lookup_list_delete] >> simp[FLOOKUP_FDIFF] >>
+      IF_CASES_TAC >> simp[] >> metis_tac[]
+      )
+    >- (
+      simp[Once minfer_cases] >> irule_at Any EQ_REFL >>
+      gvs[domain_list_insert_alt] >> goal_assum $ drule_at Any >>
+      gvs[Abbr `gens`] >> reverse $ rw[]
+      >- (
+        gvs[EVERY_MEM, MEM_GENLIST] >> ntac 2 strip_tac >> gvs[] >> conj_tac >>
+        CCONTR_TAC >> gvs[SUBSET_DEF] >> first_x_assum drule >> simp[]
+        ) >>
+      DEP_REWRITE_TAC[MAP2_MAP] >>
+      simp[LIST_TO_SET_MAP, LIST_TO_SET_FLAT] >>
+      simp[Once UNION_COMM] >> AP_TERM_TAC >>
+      simp[IMAGE_BIGUNION, IMAGE_IMAGE, LIST_TO_SET_MAP,
+           combinTheory.o_DEF, LAMBDA_PROD] >>
+      rpt (AP_TERM_TAC ORELSE AP_THM_TAC) >> ntac 2 $ rw[Once FUN_EQ_THM] >>
+      DEP_REWRITE_TAC[LIST_TO_SET_get_assumptions] >> simp[]
+      ) >>
+    gvs[new_vars_def, new_vars_constraint_def, pure_vars, pure_vars_iFunctions] >>
+    DEP_REWRITE_TAC[MAP2_MAP] >> simp[Abbr `gens`] >>
+    gvs[LIST_TO_SET_MAP, LIST_TO_SET_FLAT,
+         IMAGE_BIGUNION, IMAGE_IMAGE, LIST_TO_SET_MAP,
+         combinTheory.o_DEF, LAMBDA_PROD, MAP_GENLIST, GSYM CONJ_ASSOC] >>
+    rw[]
+    >- (
+      irule SUBSET_TRANS >> qexists_tac `BIGUNION (FRANGE mas)` >> conj_tac
+      >- (irule SUBSET_BIGUNION >> simp[FRANGE_FDIFF_SUBSET]) >>
+      rename1 `foo ⊆ _` >> gvs[SUBSET_DEF] >> rw[] >> first_x_assum drule >> rw[]
+      )
+    >- (
+      simp[pure_vars, BIGUNION_SUBSET, PULL_EXISTS] >> rpt gen_tac >>
+      PairCases_on `x` >> once_rewrite_tac[UNCURRY] >> BETA_TAC >>
+      DEP_REWRITE_TAC[LIST_TO_SET_get_assumptions] >> simp[] >> strip_tac >> gvs[] >>
+      gvs[MEM_ZIP, get_massumptions_def] >> every_case_tac >> gvs[] >>
+      gvs[BIGUNION_SUBSET, IN_FRANGE_FLOOKUP, PULL_EXISTS] >>
+      first_x_assum drule >> simp[SUBSET_DEF] >> disch_then drule >> simp[]
+      )
+    >- (rename1 `foo ⊆ _` >> gvs[SUBSET_DEF] >> rw[] >> first_x_assum drule >> rw[])
+    >- (
+      simp[LIST_TO_SET_GENLIST, IMAGE_IMAGE, combinTheory.o_DEF, pure_vars] >>
+      rw[SUBSET_DEF] >> gvs[]
+      )
+    >- (rename1 `foo ⊆ _` >> gvs[SUBSET_DEF] >> rw[] >> first_x_assum drule >> rw[])
+    )
+  >- ( (* Let *)
+    gvs[inferM_rws] >> every_case_tac >> gvs[] >>
+    pairarg_tac >> gvs[] >> every_case_tac >> gvs[] >>
+    first_x_assum drule_all >> strip_tac >> gvs[] >>
+    last_x_assum drule >> impl_tac
+    >- (rw[] >> last_x_assum drule >> simp[]) >>
+    strip_tac >> gvs[] >>
+    simp[Once minfer_cases, PULL_EXISTS] >>
+    ntac 2 $ goal_assum $ drule_at Any >> rw[]
+    >- (
+      gvs[assumptions_rel_def] >> simp[PULL_FORALL, aunion_def] >>
+      rpt gen_tac >> DEP_REWRITE_TAC[lookup_unionWith, lookup_delete] >>
+      DEP_REWRITE_TAC[cj 1 unionWith_thm, cj 2 unionWith_thm] >> simp[] >>
+      DEP_REWRITE_TAC[cj 1 delete_thm, cj 2 delete_thm] >> simp[] >>
+      simp[maunion_def, FLOOKUP_FMERGE, DOMSUB_FLOOKUP_THM] >>
+      every_case_tac >> gvs[] >> rw[] >>
+      metis_tac[wf_union, domain_union]
+      )
+    >- (
+      simp[MAP_MAP_o, combinTheory.o_DEF] >> simp[LIST_TO_SET_MAP] >>
+      imp_res_tac LIST_TO_SET_get_assumptions >> simp[]
+      )
+    >- (
+      simp[cvars_disjoint_def, DISJOINT_ALT] >> rw[] >> CCONTR_TAC >> gvs[SUBSET_DEF] >>
+      first_x_assum drule >> strip_tac >> first_x_assum drule >> strip_tac >> gvs[]
+      ) >>
+    gvs[new_vars_def, BIGUNION_FRANGE_maunion, GSYM CONJ_ASSOC] >>
+    simp[MAP_MAP_o, combinTheory.o_DEF] >>
+    simp[new_vars_constraint_def, pure_vars] >> rw[]
+    >- (rename1 `foo ⊆ _` >> gvs[SUBSET_DEF] >> rw[] >> first_x_assum drule >> rw[])
+    >- (
+      irule SUBSET_TRANS >> qexists_tac `BIGUNION (FRANGE mas)` >> conj_tac
+      >- (irule SUBSET_BIGUNION >> simp[FRANGE_DOMSUB_SUBSET]) >>
+      rename1 `foo ⊆ _` >> gvs[SUBSET_DEF] >> rw[] >> first_x_assum drule >> rw[]
+      )
+    >- (
+      simp[GSYM LIST_TO_SET_MAP, MAP_MAP_o, combinTheory.o_DEF] >>
+      simp[LIST_TO_SET_MAP] >>
+      DEP_REWRITE_TAC[LIST_TO_SET_get_assumptions] >>
+      gvs[BIGUNION_SUBSET, PULL_EXISTS, pure_vars, IN_FRANGE_FLOOKUP] >>
+      simp[get_massumptions_def] >> gen_tac >> CASE_TAC >> simp[] >>
+      strip_tac >> gvs[] >>
+      first_x_assum drule >> simp[SUBSET_DEF] >> disch_then drule >>
+      simp[] >> strip_tac >> gen_tac >> strip_tac >> gvs[SUBSET_DEF] >>
+      first_x_assum drule >> simp[]
+      )
+    >- (rename1 `foo ⊆ _` >> gvs[SUBSET_DEF] >> rw[] >> first_x_assum drule >> rw[])
+    >- (rename1 `foo ⊆ _` >> gvs[SUBSET_DEF] >> rw[] >> first_x_assum drule >> rw[])
+    >- (rename1 `foo ⊆ _` >> gvs[SUBSET_DEF] >> rw[] >> first_x_assum drule >> rw[])
+    )
+  >- ( (* Letrec *)
+    gvs[inferM_rws] >> every_case_tac >> gvs[] >>
+    pairarg_tac >> gvs[] >> every_case_tac >> gvs[] >>
+    rename [
+      `FOLDR _ _ _ _ = SOME ((tys,as,cs),m)`,
+      `infer _ _ _ _ = SOME ((ety,eas,ecs),l)`] >>
+    qsuff_tac
+      `∃ass css.
+        LIST_REL (λ((fn,e),ty) (a,c). minfer ns (domain mset) e a c ty)
+          (ZIP (fns,tys)) (ZIP (ass,css)) ∧
+        assumptions_rel as (FOLDR maunion FEMPTY ass) ∧
+        BIGUNION (set css) = set (MAP to_mconstraint cs) ∧
+        cvars_disjoint (ZIP (ass, ZIP (css, tys))) ∧
+        new_vars (FOLDR maunion FEMPTY ass)
+          (BIGUNION (set css)) (iFunctions tys Exception) ⊆ {v | l ≤ v ∧ v < m} ∧
+        LENGTH fns = LENGTH tys ∧ LENGTH ass = LENGTH css ∧
+        l ≤ m`
+    >- (
+      rw[] >> gvs[] >>
+      first_x_assum drule >> impl_tac >- (rw[] >> first_x_assum drule >> rw[]) >>
+      strip_tac >> gvs[] >>
+      simp[Once minfer_cases, PULL_EXISTS] >>
+      rpt $ goal_assum $ drule_at Any >> simp[] >>
+      DEP_REWRITE_TAC[MAP2_MAP] >>
+      simp[MAP_MAP_o, combinTheory.o_DEF, LAMBDA_PROD] >>
+      gvs[new_vars_def, LIST_TO_SET_MAP, IMAGE_IMAGE,
+          combinTheory.o_DEF, LAMBDA_PROD, pure_vars] >>
+      gvs[pure_vars_iFunctions, BIGUNION_SUBSET, MEM_MAP, PULL_EXISTS,
+          LAMBDA_PROD, MEM_FLAT, pure_vars, EXISTS_PROD] >>
+      simp[PULL_FORALL] >> rpt gen_tac >>
+      DEP_REWRITE_TAC[MEM_ZIP] >> simp[PULL_EXISTS] >> rw[]
+      >- (
+        gvs[assumptions_rel_def, aunion_def] >>
+        simp[PULL_FORALL] >> rpt gen_tac >>
+        DEP_REWRITE_TAC[lookup_list_delete, lookup_unionWith] >>
+        DEP_REWRITE_TAC[cj 1 map_ok_list_delete, cj 2 map_ok_list_delete] >>
+        DEP_REWRITE_TAC[cj 1 unionWith_thm, cj 2 unionWith_thm] >> simp[] >>
+        gvs[maunion_def, FLOOKUP_FDIFF, FLOOKUP_FMERGE, IN_FRANGE_FLOOKUP] >>
+        simp[MEM_MAP, EXISTS_PROD] >> gvs[PULL_EXISTS] >>
+        IF_CASES_TAC >> gvs[]
+        >- (rw[] >> every_case_tac >> gvs[] >> metis_tac[wf_union]) >>
+        rw[] >> every_case_tac >> gvs[] >> metis_tac[wf_union, domain_union]
+        )
+      >- (
+        simp[AC UNION_ASSOC UNION_COMM] >> rpt (AP_TERM_TAC ORELSE AP_THM_TAC) >>
+        simp[LIST_TO_SET_FLAT, MAP_MAP_o, combinTheory.o_DEF, LAMBDA_PROD,
+             IMAGE_BIGUNION, LIST_TO_SET_MAP, IMAGE_IMAGE] >>
+        rpt (AP_TERM_TAC ORELSE AP_THM_TAC) >>
+        rewrite_tac[FUN_EQ_THM] >> rpt gen_tac >> BETA_TAC >>
+        rpt (AP_TERM_TAC ORELSE AP_THM_TAC) >>
+        irule LIST_TO_SET_get_assumptions >>
+        gvs[assumptions_rel_def, aunion_def] >>
+        simp[PULL_FORALL] >> rpt gen_tac >>
+        DEP_REWRITE_TAC[lookup_unionWith] >>
+        DEP_REWRITE_TAC[cj 1 unionWith_thm, cj 2 unionWith_thm] >> simp[] >>
+        gvs[maunion_def, FLOOKUP_FMERGE, IN_FRANGE_FLOOKUP] >>
+        rw[] >> every_case_tac >> gvs[] >> metis_tac[wf_union, domain_union]
+        )
+      >- (
+        gvs[cvars_disjoint_def] >>
+        once_rewrite_tac[CONS_APPEND] >> rewrite_tac[list_disjoint_append] >>
+        simp[MEM_MAP, EXISTS_PROD, PULL_EXISTS] >> rpt gen_tac >>
+        DEP_REWRITE_TAC[MEM_ZIP] >> DEP_REWRITE_TAC[cj 1 LENGTH_ZIP] >> simp[] >>
+        imp_res_tac LIST_REL_LENGTH >> gvs[] >> simp[PULL_EXISTS] >> rw[] >>
+        pop_assum mp_tac >> DEP_REWRITE_TAC[EL_ZIP] >> simp[] >> strip_tac >> gvs[] >>
+        irule SUBSET_DISJOINT >>
+        qexistsl_tac [`{v | n ≤ v ∧ v < l}`,`{v | l ≤ v ∧ v < m}`] >>
+        conj_tac >- rw[DISJOINT_ALT] >> gvs[] >>
+        simp[new_vars_def, BIGUNION_SUBSET, IMAGE_IMAGE, PULL_EXISTS] >> rw[]
+        >- (
+          gvs[IN_FRANGE_FLOOKUP, FLOOKUP_FOLDR_maunion, PULL_EXISTS,
+              FLOOKUP_DEF, BIGUNION_SUBSET] >>
+          first_x_assum irule >> simp[EL_MEM] >>
+          goal_assum $ drule_at Any >> simp[EL_MEM]
+          )
+        >- (
+          qpat_x_assum `BIGUNION _ = _` mp_tac >> simp[EXTENSION] >>
+          disch_then $ mp_tac o iffLR >> simp[PULL_EXISTS] >>
+          disch_then drule >> simp[EL_MEM] >> strip_tac >> gvs[]
+          )
+        >- (last_x_assum irule >> simp[EL_MEM])
+        )
+      >- (
+        drule $ SIMP_RULE std_ss [SUBSET_DEF] FRANGE_FDIFF_SUBSET >>
+        simp[Once maunion_def] >> gvs[IN_FRANGE_FLOOKUP, FLOOKUP_FMERGE] >> rw[] >>
+        every_case_tac >> gvs[PULL_EXISTS]
+        >- (first_x_assum drule >> rw[SUBSET_DEF] >> first_x_assum drule >> simp[])
+        >- (first_x_assum drule >> rw[SUBSET_DEF] >> first_x_assum drule >> simp[])
+        >- (
+          first_x_assum drule >> first_x_assum drule >>
+          rw[SUBSET_DEF] >> first_x_assum drule >> simp[]
+          )
+        )
+      >- (
+        gvs[get_assumptions_def, assumptions_rel_def] >> every_case_tac >> gvs[] >>
+        gvs[miscTheory.toAList_domain] >>
+        qpat_x_assum `lookup _ _ = _` mp_tac >> simp[aunion_def] >>
+        DEP_REWRITE_TAC[lookup_unionWith] >> simp[] >>
+        ntac 3 $ first_x_assum $ qspec_then `p_1` assume_tac >>
+        rw[] >> every_case_tac >> gvs[IN_FRANGE_FLOOKUP, PULL_EXISTS]
+        >- (first_x_assum drule >> simp[SUBSET_DEF])
+        >- (first_x_assum drule >> simp[SUBSET_DEF] >> disch_then drule >> simp[])
+        >- (
+          gvs[domain_union] >>
+          first_x_assum drule >> first_x_assum drule >> simp[SUBSET_DEF] >>
+          rw[] >> first_x_assum drule >> simp[]
+          )
+        )
+      >- (
+        gvs[get_assumptions_def, assumptions_rel_def] >> every_case_tac >> gvs[] >>
+        gvs[miscTheory.toAList_domain] >>
+        qpat_x_assum `lookup _ _ = _` mp_tac >> simp[aunion_def] >>
+        DEP_REWRITE_TAC[lookup_unionWith] >> simp[] >>
+        ntac 3 $ first_x_assum $ qspec_then `p_1` assume_tac >>
+        rw[] >> every_case_tac >> gvs[IN_FRANGE_FLOOKUP, PULL_EXISTS]
+        >- (first_x_assum drule >> simp[SUBSET_DEF] >> disch_then drule >> simp[])
+        >- (first_x_assum drule >> simp[SUBSET_DEF] >> disch_then drule >> simp[])
+        >- (
+          gvs[domain_union] >>
+          first_x_assum drule >> first_x_assum drule >> simp[SUBSET_DEF] >>
+          rw[] >> first_x_assum drule >> simp[]
+          )
+        )
+      >- (
+        last_x_assum $ qspec_then `EL n'' tys` mp_tac >> simp[EL_MEM, SUBSET_DEF] >>
+        rw[] >> first_x_assum drule >> simp[]
+        )
+      >- (
+        last_x_assum drule >> simp[SUBSET_DEF] >> rw[] >> first_x_assum drule >> simp[]
+        )
+      >- (
+        last_x_assum drule >> simp[SUBSET_DEF] >> rw[] >> first_x_assum drule >> simp[]
+        )
+      >- (gvs[SUBSET_DEF] >> rw[] >> first_x_assum drule >> simp[])
+      ) >>
+    qpat_x_assum `FOLDR _ _ _ _ = _` mp_tac >>
+    `∀mvar. mvar ∈ domain mset ⇒ mvar < l` by (
+      first_x_assum drule_all >> strip_tac >> gvs[] >> rw[] >>
+      first_x_assum drule >> simp[]) >>
+    pop_assum mp_tac >> ntac 2 $ pop_assum kall_tac >>
+    last_x_assum mp_tac >> last_x_assum kall_tac >>
+    rename1 `n ≤ m` >>
+    map_every qid_spec_tac [`m`,`l`,`tys`,`as`,`cs`] >>
+    Induct_on `fns` >> rw[] >> simp[]
+    >- (
+      qexistsl_tac [`[]`,`[]`] >> simp[assumptions_rel_def, iFunctions_def] >>
+      simp[cvars_disjoint_def, new_vars_def, list_disjoint_def, pure_vars]
+      ) >>
+    every_case_tac >> gvs[PULL_EXISTS, EXISTS_PROD] >>
+    pairarg_tac >> gvs[] >> every_case_tac >> gvs[] >> simp[PULL_EXISTS] >>
+    rename1 `FOLDR _ _ _ _ = SOME ((tysrest,asrest,csrest),r)` >>
+    rename1 `infer _ _ _ _ = SOME ((ty,as,cs),m)` >>
+    gvs[DISJ_IMP_THM, FORALL_AND_THM] >>
+    first_x_assum drule >> strip_tac >> gvs[] >>
+    last_x_assum drule >> impl_tac >- (rw[] >> first_x_assum drule >> rw[]) >>
+    strip_tac >> gvs[] >>
+    qexistsl_tac [`mas::ass`,`set (MAP to_mconstraint cs)::css`] >> rw[]
+    >- (
+      gvs[assumptions_rel_def, aunion_def, PULL_FORALL] >> rpt gen_tac >>
+      DEP_REWRITE_TAC[cj 1 unionWith_thm, cj 2 unionWith_thm, lookup_unionWith] >>
+      gvs[maunion_def, FLOOKUP_FMERGE] >>
+      rw[] >> every_case_tac >> gvs[] >> metis_tac[wf_union, domain_union, UNION_COMM]
+      )
+    >- (
+      gvs[cvars_disjoint_def] >>
+      once_rewrite_tac[CONS_APPEND] >> rewrite_tac[list_disjoint_append] >>
+      simp[MEM_MAP, EXISTS_PROD, PULL_EXISTS] >> rpt gen_tac >>
+      DEP_REWRITE_TAC[MEM_ZIP] >> DEP_REWRITE_TAC[cj 1 LENGTH_ZIP] >> simp[] >>
+      imp_res_tac LIST_REL_LENGTH >> gvs[] >> simp[PULL_EXISTS] >> rw[] >>
+      pop_assum mp_tac >> DEP_REWRITE_TAC[EL_ZIP] >> simp[] >> strip_tac >> gvs[] >>
+      irule SUBSET_DISJOINT >> goal_assum $ drule_at Any >>
+      qexists_tac `{v | n ≤ v ∧ v < r}` >>
+      conj_tac >- rw[DISJOINT_ALT] >> gvs[] >>
+      irule SUBSET_TRANS >> goal_assum $ drule_at Any >>
+      gvs[new_vars_def, BIGUNION_SUBSET, pure_vars, PULL_EXISTS] >> rw[]
+      >- (
+        simp[SUBSET_DEF] >> rw[] >> disj1_tac >> disj1_tac >>
+        gvs[IN_FRANGE_FLOOKUP, FLOOKUP_FOLDR_maunion, PULL_EXISTS,
+            GSYM CONJ_ASSOC, FLOOKUP_DEF, BIGUNION_SUBSET] >>
+        rpt $ goal_assum $ drule_at Any >> simp[EL_MEM]
+        )
+      >- (
+        simp[SUBSET_DEF] >> rw[] >> disj1_tac >> disj2_tac >>
+        simp[PULL_EXISTS] >> goal_assum drule >>
+        qpat_x_assum `BIGUNION _ = _` mp_tac >> simp[EXTENSION] >>
+        disch_then $ irule o iffLR >> goal_assum drule >> simp[EL_MEM]
+        )
+      >- (
+        simp[SUBSET_DEF] >> rw[] >> disj2_tac >> simp[MEM_MAP, PULL_EXISTS] >>
+        simp[pure_vars_iFunctions, pure_vars] >>
+        simp[MEM_MAP, PULL_EXISTS] >> goal_assum drule >> simp[EL_MEM]
+        )
+      )
+    >- (
+      gvs[new_vars_def, BIGUNION_FRANGE_maunion, GSYM CONJ_ASSOC,
+          pure_vars, pure_vars_iFunctions] >> rw[] >>
+      rename1 `foo ⊆ _` >> gvs[SUBSET_DEF] >> rw[] >> first_x_assum drule >> rw[]
+      )
+    )
+  >- gvs[fail_def] (* Case empty case *)
+  >- ( (* Case non-empty case *)
+    Cases_on `css` >- gvs[inferM_rws] >>
+    Cases_on `∃pvars rest. h::t = [("",pvars,rest)]`
+    >- ( (* TupleCase *)
+      gvs[] >> gvs[inferM_rws] >> every_case_tac >> gvs[] >>
+      pairarg_tac >> gvs[] >> every_case_tac >> gvs[] >>
+      rename1 `infer _ _ _ _ = SOME ((ety,eas,ecs),m)` >>
+      rename1 `SOME ((tyrest,_,_),r)` >>
+      first_x_assum drule >> impl_tac
+      >- (
+        simp[domain_list_insert] >> rw[] >> gvs[MEM_GENLIST] >>
+        first_x_assum drule >> simp[]
+        ) >>
+      strip_tac >> gvs[] >> first_x_assum drule >> impl_tac
+      >- (rw[] >> first_x_assum drule >> simp[]) >>
+      strip_tac >> gvs[] >>
+      simp[Once minfer_cases] >> irule_at Any OR_INTRO_THM1 >> simp[PULL_EXISTS] >>
+      DEP_REWRITE_TAC[MAP2_MAP] >>
+      simp[MAP2_MAP, MAP_FLAT, MAP_MAP_o, combinTheory.o_DEF, LAMBDA_PROD,
+           LIST_TO_SET_MAP, LIST_TO_SET_FLAT, IMAGE_IMAGE, IMAGE_BIGUNION] >>
+      qexistsl_tac [
+        `mas'`,`mas`,`IMAGE to_mconstraint (set ecs ∪ set csrest)`,
+        `IMAGE to_mconstraint (set csrest)`, `mas'`,
+        `IMAGE to_mconstraint (set ecs)`,`ety`,`n`,
+        `GENLIST (λn'. n' + SUC n) (LENGTH pvars)`] >>
+      rw[] >> gvs[LIST_TO_SET_MAP]
+      >- (
+        simp[AC UNION_ASSOC UNION_COMM] >> rpt (AP_TERM_TAC ORELSE AP_THM_TAC) >>
+        imp_res_tac LIST_TO_SET_get_assumptions >> simp[] >>
+        rpt (AP_TERM_TAC ORELSE AP_THM_TAC) >> simp[MAP2_MAP, LIST_TO_SET_MAP]
+        )
+      >- gvs[domain_list_insert_alt, INSERT_UNION_EQ]
+      >- (CCONTR_TAC >> gvs[] >> first_x_assum drule >> simp[])
+      >- (CCONTR_TAC >> gvs[SUBSET_DEF] >> first_x_assum drule >> simp[])
+      >- (CCONTR_TAC >> gvs[SUBSET_DEF] >> first_x_assum drule >> simp[])
+      >- (
+        simp[EVERY_MEM, MEM_GENLIST, PULL_EXISTS] >> rw[] >> gvs[SUBSET_DEF] >>
+        CCONTR_TAC >> gvs[] >> first_x_assum drule >> simp[]
+        )
+      >- (
+        gvs[assumptions_rel_def, aunion_def] >> simp[PULL_FORALL] >> rpt gen_tac >>
+        DEP_REWRITE_TAC[lookup_unionWith, lookup_list_delete] >>
+        DEP_REWRITE_TAC[cj 1 unionWith_thm, cj 2 unionWith_thm] >>
+        DEP_REWRITE_TAC[cj 1 map_ok_list_delete, cj 2 map_ok_list_delete] >>
+        simp[maunion_def, FLOOKUP_FMERGE, FLOOKUP_FDIFF] >>
+        rw[] >> every_case_tac >> gvs[] >> metis_tac[domain_union, wf_union]
+        ) >>
+      gvs[new_vars_def, BIGUNION_FRANGE_maunion, GSYM CONJ_ASSOC,
+          pure_vars, MAP_MAP_o, combinTheory.o_DEF, MAP_GENLIST,
+          LIST_TO_SET_GENLIST, IMAGE_IMAGE, GSYM INSERT_SING_UNION,
+          IMAGE_BIGUNION, LAMBDA_PROD] >> rw[]
+      >- (rename1 `foo ⊆ _` >> gvs[SUBSET_DEF] >> rw[] >> first_x_assum drule >> rw[])
+      >- (
+        gvs[BIGUNION_SUBSET] >> rw[] >>
+        drule $ SIMP_RULE std_ss [SUBSET_DEF] FRANGE_FDIFF_SUBSET >> strip_tac >>
+        first_x_assum drule >> simp[SUBSET_DEF] >> rw[] >> first_x_assum drule >> rw[]
+        )
+      >- (rename1 `foo ⊆ _` >> gvs[SUBSET_DEF] >> rw[] >> first_x_assum drule >> rw[])
+      >- (rename1 `foo ⊆ _` >> gvs[SUBSET_DEF] >> rw[] >> first_x_assum drule >> rw[])
+      >- simp[BIGUNION_SUBSET, PULL_EXISTS]
+      >- (
+        gvs[BIGUNION_SUBSET, IN_FRANGE_FLOOKUP, PULL_EXISTS] >>
+        gvs[get_assumptions_def, assumptions_rel_def, PULL_EXISTS] >>
+        gen_tac >> strip_tac >> every_case_tac >> gvs[] >>
+        gvs[miscTheory.toAList_domain] >>
+        first_x_assum drule >> simp[SUBSET_DEF] >> disch_then drule >> simp[]
+        )
+      >- (
+        gvs[BIGUNION_SUBSET, EXISTS_PROD, PULL_EXISTS, MEM_ZIP, pure_vars] >>
+        gvs[IN_FRANGE_FLOOKUP, get_assumptions_def, assumptions_rel_def, PULL_EXISTS] >>
+        ntac 2 gen_tac >> strip_tac >> every_case_tac >> gvs[] >>
+        gvs[miscTheory.toAList_domain] >>
+        first_x_assum drule >> simp[SUBSET_DEF] >> disch_then drule >> simp[]
+        )
+      >- (
+        gvs[BIGUNION_SUBSET, PULL_EXISTS, SUBSET_DEF] >> rw[] >>
+        first_x_assum drule_all >> simp[]
+        )
+      >- (
+        gvs[BIGUNION_SUBSET, PULL_EXISTS, SUBSET_DEF] >> rw[] >>
+        first_x_assum drule_all >> simp[]
+        )
+      >- (gvs[SUBSET_DEF] >> rw[] >> first_x_assum drule_all >> simp[])
+      ) >>
+    qpat_abbrev_tac `cases = h::t` >>
+    qmatch_asmsub_abbrev_tac `list_CASE _ _ (λv1 v2. foo)` >>
+    `foo n = SOME ((ty,as,cs),m)` by (PairCases_on `h` >> gvs[Abbr `cases`] >>
+      Cases_on `h0` >> gvs[] >> Cases_on `t` >> gvs[]) >>
+    qpat_x_assum `(list_CASE _ _ _) _ = _` kall_tac >> gvs[Abbr `foo`] >>
+    `∀n' ty' as' cs' m'.
+      infer ns mset e n' = SOME ((ty',as',cs'),m') ∧
+      (∀mvar. mvar ∈ domain mset ⇒ mvar < n') ⇒
+      ∃mas.
+        assumptions_rel as' mas ∧
+        minfer ns (domain mset) e mas (set (MAP to_mconstraint cs'))
+          ty' ∧ n' ≤ m' ∧
+        new_vars mas (set (MAP to_mconstraint cs')) ty' ⊆
+        {v | n' ≤ v ∧ v < m'}` by (
+        unabbrev_all_tac >> PairCases_on `h` >> gvs[] >>
+        Cases_on `h0` >> gvs[] >> Cases_on `t` >> gvs[]) >>
+    `∀fresh_v fresh_tyargs cname pvars rest.
+      MEM (cname,pvars,rest) cases ⇒
+        ∀n' ty' as' cs' m'.
+          infer ns (list_insert (fresh_v::fresh_tyargs) mset) rest n' =
+          SOME ((ty',as',cs'),m') ∧
+          (∀mvar.
+             mvar ∈ domain (list_insert (fresh_v::fresh_tyargs) mset) ⇒
+             mvar < n') ⇒
+          ∃mas.
+            assumptions_rel as' mas ∧
+            minfer ns (domain (list_insert (fresh_v::fresh_tyargs) mset))
+              rest mas (set (MAP to_mconstraint cs')) ty' ∧ n' ≤ m' ∧
+            new_vars mas (set (MAP to_mconstraint cs')) ty' ⊆
+            {v | n' ≤ v ∧ v < m'}` by (
+        unabbrev_all_tac >> PairCases_on `h` >> gvs[] >>
+        Cases_on `h0` >> gvs[] >> Cases_on `t` >> gvs[] >>
+        rw[] >> first_x_assum irule >> simp[] >> metis_tac[]) >>
+    last_x_assum assume_tac >> ntac 4 $ last_x_assum kall_tac >>
+    qpat_x_assum `_ = SOME _` assume_tac >> gvs[inferM_rws] >>
+    qmatch_asmsub_abbrev_tac `oreturn foo` >>
+    Cases_on `foo` >> gvs[inferM_rws] >> rename1 `SOME tdef` >>
+    pairarg_tac >> gvs[inferM_rws] >> every_case_tac >> gvs[] >>
+    gvs[ALOOKUP_MAP, MAP_MAP_o, combinTheory.o_DEF, SF ETA_ss] >>
+    qmatch_asmsub_abbrev_tac `FOLDR f` >>
+    rename [
+      `infer _ _ _ _ = SOME ((ety,eas,ecs),m)`,
+      `FOLDR _ _ _ _ = SOME ((tyrest,asrest,csrest),l)`] >>
+    drule get_typedef_SOME >>
+    disch_then $ qspec_then `FST ns` assume_tac >> gvs[] >>
+    `EVERY (λ(cn,pvs,_).
+      MEM (cn, LENGTH pvs) (MAP (λ(cn,ts). (cn, LENGTH ts)) cdefs)) cases` by (
+      rw[EVERY_MEM] >> pairarg_tac >> simp[] >>
+      drule $ iffRL sortingTheory.PERM_MEM_EQ >>
+      simp[MEM_MAP, PULL_EXISTS, EXISTS_PROD] >> rw[] >>
+      first_x_assum drule >> simp[]) >>
+    `ALL_DISTINCT (MAP FST cdefs)` by (
+      qpat_x_assum `namespace_ok _` assume_tac >> PairCases_on `ns` >>
+      gvs[namespace_ok_def] >> gvs[ALL_DISTINCT_APPEND, MAP_FLAT] >>
+      drule miscTheory.ALL_DISTINCT_FLAT_EVERY >>
+      simp[EVERY_EL, EL_MAP] >> gvs[oEL_THM] >>
+      disch_then drule >> simp[]) >>
+    qsuff_tac
+      `∃ass css final_as final_cs.
+        LIST_REL (λ((cname,pvars,rest),ty) (a,c).
+          minfer ns (n INSERT set (GENLIST (λn'. n' + SUC n) ar) ∪ domain mset)
+            rest a c ty)
+          (ZIP (cases,tyrest)) (ZIP (ass,css)) ∧
+        LIST_REL
+         (λ((cn,pvars,rest),as,cs) (as',cs').
+              ∃schemes.
+                ALOOKUP cdefs cn = SOME schemes ∧
+                (let pvar_cs =
+                  MAP2 (λv t. IMAGE (λn. mUnify (CVar n) t) (get_massumptions as v))
+                    (v::pvars)
+                    (CVar n::
+                      MAP (isubst (MAP CVar (GENLIST (λn'. n' + SUC n) ar)) ∘ itype_of)
+                        schemes)
+                 in
+                   as' = FDIFF as (v INSERT set pvars) ∧
+                   cs' = BIGUNION (set pvar_cs) ∪ cs))
+         (ZIP (cases,ZIP (ass,css))) (ZIP (final_as,final_cs)) ∧
+        assumptions_rel asrest (FOLDR maunion FEMPTY final_as) ∧
+        BIGUNION (set final_cs) = set (MAP to_mconstraint csrest) ∧
+        cvars_disjoint (ZIP (ass, ZIP (css, tyrest))) ∧
+        new_vars (FOLDR maunion FEMPTY ass)
+          (BIGUNION (set css)) (iFunctions tyrest Exception) ⊆
+            {v | ar + SUC n ≤ v ∧ v < l} ∧
+        LENGTH cases = LENGTH tyrest ∧ LENGTH ass = LENGTH css ∧
+        LENGTH final_as = LENGTH final_cs ∧ ar + SUC n ≤ l`
+    >- (
+      rw[] >> gvs[] >>
+      last_x_assum drule >> impl_tac >- (rw[] >> first_x_assum drule >> simp[]) >>
+      strip_tac >> gvs[] >>
+      simp[Once minfer_cases, PULL_EXISTS, GSYM CONJ_ASSOC] >>
+      goal_assum $ drule_at $ Pat `LIST_REL _ _ _` >>
+      gvs[domain_list_insert_alt, INSERT_UNION_EQ] >>
+      goal_assum $ drule_at $ Pat `LIST_REL _ _ _` >>
+      rpt $ goal_assum $ drule_at Any >> simp[SF ETA_ss, combinTheory.o_DEF] >>
+      gvs[MAP_MAP_o, combinTheory.o_DEF, LAMBDA_PROD, new_vars_def,
+          LIST_TO_SET_MAP, IMAGE_IMAGE, pure_vars, pure_vars_iFunctions,
+          BIGUNION_SUBSET, PULL_EXISTS, MEM_GENLIST, EXISTS_PROD] >>
+      rw[]
+      >- (
+        gvs[assumptions_rel_def, aunion_def] >> simp[PULL_FORALL] >> rpt gen_tac >>
+        DEP_REWRITE_TAC[lookup_unionWith] >>
+        DEP_REWRITE_TAC[cj 1 unionWith_thm, cj 2 unionWith_thm] >> simp[] >>
+        simp[Once maunion_def, FLOOKUP_FMERGE] >>
+        rw[] >> every_case_tac >> gvs[] >> metis_tac[wf_union, domain_union]
+        )
+      >- (
+        gvs[cvars_disjoint_def] >>
+        once_rewrite_tac[CONS_APPEND] >> rewrite_tac[list_disjoint_append] >>
+        simp[MEM_MAP, EXISTS_PROD, PULL_EXISTS] >> rpt gen_tac >>
+        DEP_REWRITE_TAC[MEM_ZIP] >> DEP_REWRITE_TAC[cj 1 LENGTH_ZIP] >> simp[] >>
+        imp_res_tac LIST_REL_LENGTH >> gvs[] >> simp[PULL_EXISTS] >> rw[] >>
+        pop_assum mp_tac >> DEP_REWRITE_TAC[EL_ZIP] >> simp[] >> strip_tac >> gvs[] >>
+        irule SUBSET_DISJOINT >>
+        qexistsl_tac [`{v | l ≤ v ∧ v < m}`,`{v | n ≤ v ∧ v < l}`] >>
+        conj_tac >- rw[DISJOINT_ALT] >> gvs[] >>
+        simp[new_vars_def, BIGUNION_SUBSET, IMAGE_IMAGE, PULL_EXISTS] >> rw[]
+        >- (
+          gvs[IN_FRANGE_FLOOKUP, FLOOKUP_FOLDR_maunion, PULL_EXISTS,
+              FLOOKUP_DEF, BIGUNION_SUBSET] >>
+          first_x_assum $ drule_at Any >> disch_then $ drule_at Any >>
+          simp[EL_MEM, SUBSET_DEF] >> rw[] >>
+          first_x_assum drule >> simp[]
+          )
+        >- (
+          first_x_assum drule >> simp[EL_MEM, SUBSET_DEF] >> rw[] >>
+          first_x_assum drule >> simp[]
+          )
+        >- (
+          gvs[SUBSET_DEF, PULL_FORALL] >> gen_tac >> strip_tac >>
+          qpat_x_assum `∀a b. MEM _ tyrest ⇒ _` $ drule_at Any >> simp[EL_MEM]
+          )
+        )
+      >- (CCONTR_TAC >> gvs[SUBSET_DEF] >> first_x_assum drule_all >> simp[])
+      >- (CCONTR_TAC >> gvs[SUBSET_DEF] >> first_x_assum drule_all >> simp[])
+      >- (CCONTR_TAC >> gvs[SUBSET_DEF] >> first_x_assum drule_all >> simp[])
+      >- (CCONTR_TAC >> gvs[SUBSET_DEF] >> first_x_assum drule_all >> simp[])
+      >- (
+        simp[EVERY_MEM, FORALL_PROD] >> rpt gen_tac >>
+        DEP_REWRITE_TAC[MEM_ZIP] >> simp[] >>
+        imp_res_tac LIST_REL_LENGTH >> gvs[LENGTH_ZIP] >> simp[PULL_EXISTS] >>
+        gen_tac >> strip_tac >>
+        pop_assum mp_tac >> DEP_REWRITE_TAC[EL_ZIP] >> simp[] >>
+        strip_tac >> gvs[] >>
+        gvs[IN_FRANGE_FLOOKUP, FLOOKUP_FOLDR_maunion, PULL_EXISTS,
+            BIGUNION_SUBSET, FLOOKUP_DEF, GSYM CONJ_ASSOC] >>
+        rw[]
+        >- (
+          CCONTR_TAC >> gvs[] >>
+          first_x_assum $ drule_at Any >> disch_then $ drule_at Any >>
+          simp[EL_MEM, SUBSET_DEF] >> goal_assum drule >> simp[]
+          )
+        >- (
+          CCONTR_TAC >> gvs[] >> first_x_assum $ drule_at Any >>
+          simp[EL_MEM, SUBSET_DEF] >> goal_assum drule >> simp[]
+          )
+        >- (
+          CCONTR_TAC >> gvs[SUBSET_DEF] >>
+          first_x_assum $ drule_at Any >> simp[EL_MEM]
+          )
+        )
+      >- (
+        simp[EVERY_MEM, FORALL_PROD, MEM_GENLIST] >> rpt gen_tac >>
+        gvs[IN_FRANGE_FLOOKUP, FLOOKUP_FOLDR_maunion, PULL_EXISTS,
+            BIGUNION_SUBSET, FLOOKUP_DEF, GSYM CONJ_ASSOC] >>
+        gen_tac >> strip_tac >> gvs[] >> rpt conj_tac
+        >- (CCONTR_TAC >> gvs[] >> first_x_assum drule >> simp[])
+        >- (CCONTR_TAC >> gvs[SUBSET_DEF] >> first_x_assum $ drule_at Any >> simp[])
+        >- (
+          CCONTR_TAC >> gvs[SUBSET_DEF, PULL_FORALL] >>
+          first_x_assum drule_all >> simp[]
+          )
+        >- (CCONTR_TAC >> gvs[SUBSET_DEF] >> first_x_assum $ drule_at Any >> simp[]) >>
+        rpt gen_tac >> DEP_REWRITE_TAC[MEM_ZIP] >> simp[] >>
+        imp_res_tac LIST_REL_LENGTH >> gvs[] >> strip_tac >> gvs[] >>
+        pop_assum mp_tac >> DEP_REWRITE_TAC[EL_ZIP] >> simp[] >>
+        strip_tac >> gvs[SUBSET_DEF, PULL_FORALL, GSYM CONJ_ASSOC, AND_IMP_INTRO] >>
+        rw[]
+        >- (
+          CCONTR_TAC >> gvs[] >>
+          first_x_assum $ drule_at Any >> disch_then $ drule_at Any >> simp[EL_MEM]
+          )
+        >- (
+          CCONTR_TAC >> gvs[] >>
+          first_x_assum $ drule_at Any >> disch_then $ drule_at Any >> simp[EL_MEM]
+          )
+        >- (
+          CCONTR_TAC >> gvs[SUBSET_DEF] >>
+          first_x_assum $ drule_at Any >> simp[EL_MEM]
+          )
+        )
+      >- (
+        gvs[IN_FRANGE_FLOOKUP, PULL_EXISTS, BIGUNION_SUBSET] >>
+        pop_assum mp_tac >> simp[Once maunion_def, FLOOKUP_FMERGE] >>
+        rw[] >> every_case_tac >> gvs[SUBSET_DEF, PULL_FORALL]
+        >- (first_x_assum drule >> rw[] >> first_x_assum drule >> simp[])
+        >- (
+          gen_tac >> strip_tac >> gvs[FLOOKUP_FOLDR_maunion] >>
+          qpat_x_assum `MEM _ _` mp_tac >> simp[MEM_EL] >> strip_tac >>
+          gvs[LIST_REL_EL_EQN] >> first_x_assum drule >> simp[EL_ZIP] >>
+          pairarg_tac >> gvs[] >> strip_tac >> gvs[] >>
+          gvs[FLOOKUP_FDIFF, PULL_EXISTS, FLOOKUP_DEF, GSYM CONJ_ASSOC] >>
+          first_x_assum $ drule_at Any >> simp[EL_MEM] >>
+          disch_then $ drule_at Any >> simp[EL_MEM]
+          )
+        >- (
+          rpt gen_tac >> first_x_assum drule >> strip_tac >> conj_tac
+          >- (strip_tac >> first_x_assum drule >> simp[]) >>
+          gvs[FLOOKUP_FOLDR_maunion] >> strip_tac >> gvs[] >>
+          qpat_x_assum `MEM _ _` mp_tac >> simp[MEM_EL] >> strip_tac >>
+          gvs[LIST_REL_EL_EQN] >> first_x_assum drule >> simp[EL_ZIP] >>
+          pairarg_tac >> gvs[] >> strip_tac >> gvs[] >>
+          gvs[FLOOKUP_FDIFF, PULL_EXISTS, FLOOKUP_DEF, GSYM CONJ_ASSOC] >>
+          first_x_assum $ drule_at Any >> simp[EL_MEM] >>
+          disch_then $ drule_at Any >> simp[EL_MEM] >>
+          disch_then drule >> simp[]
+          )
+        )
+      >- (gvs[SUBSET_DEF] >> rw[] >> first_x_assum drule >> simp[])
+      >- (gvs[SUBSET_DEF] >> rw[] >> first_x_assum drule >> simp[])
+      >- (
+        gvs[SUBSET_DEF] >> gen_tac >> strip_tac >>
+        Cases_on `tyrest` >> gvs[DISJ_IMP_THM, FORALL_AND_THM] >>
+        first_x_assum drule >> simp[]
+        )
+      >- (
+        gvs[SUBSET_DEF] >> gen_tac >> strip_tac >>
+        Cases_on `tyrest` >> gvs[DISJ_IMP_THM, FORALL_AND_THM] >>
+        first_x_assum drule_all >> simp[]
+        )
+      >- (gvs[SUBSET_DEF] >> rw[] >> first_x_assum drule_all >> simp[])
+      >- (
+        qpat_assum `BIGUNION _ = _` mp_tac >> rewrite_tac[EXTENSION] >> simp[] >>
+        disch_then $ mp_tac o iffRL >> simp[PULL_EXISTS] >>
+        disch_then drule >> strip_tac >> gvs[] >>
+        qpat_x_assum `MEM _ _` mp_tac >> simp[MEM_EL] >> strip_tac >> gvs[] >>
+        qpat_x_assum `LIST_REL _ _ _` assume_tac >> gvs[LIST_REL_EL_EQN] >>
+        first_x_assum drule >> simp[EL_ZIP] >> pairarg_tac >> gvs[] >>
+        strip_tac >> gvs[pure_vars]
+        >- (
+          gvs[get_massumptions_def] >> every_case_tac >> gvs[] >>
+          gvs[IN_FRANGE_FLOOKUP, PULL_EXISTS, FLOOKUP_FOLDR_maunion, FLOOKUP_DEF] >>
+          first_x_assum $ drule_at Any >>
+          simp[EL_MEM, BIGUNION_SUBSET, PULL_EXISTS] >>
+          disch_then $ drule_at Any >> simp[EL_MEM, SUBSET_DEF] >>
+          disch_then drule >> simp[]
+          )
+        >- (
+          qpat_x_assum `MEM _ (MAP2 _ _ _)` mp_tac >>
+          DEP_REWRITE_TAC[MAP2_MAP] >> simp[] >>
+          gvs[EVERY_EL] >> last_x_assum drule >> simp[] >> strip_tac >> gvs[] >>
+          drule_all ALOOKUP_ALL_DISTINCT_MEM >> simp[] >> strip_tac >> gvs[] >>
+          simp[MEM_MAP, EXISTS_PROD, MEM_ZIP, PULL_EXISTS] >> rw[] >>
+          gvs[pure_vars, EL_MAP] >> conj_tac
+          >- (
+            qpat_x_assum `_ ∈ get_massumptions _ _` mp_tac >>
+            simp[get_massumptions_def] >> CASE_TAC >> gvs[] >> strip_tac >>
+            gvs[IN_FRANGE_FLOOKUP, FLOOKUP_FOLDR_maunion, PULL_EXISTS,
+                BIGUNION_SUBSET, FLOOKUP_DEF] >>
+            first_x_assum $ drule_at Any >> disch_then $ drule_at Any >>
+            simp[EL_MEM, SUBSET_DEF] >> disch_then drule >> simp[]
+            )
+          >- (
+            irule SUBSET_TRANS >>
+            irule_at Any pure_vars_isubst_SUBSET >> simp[] >>
+            simp[BIGUNION_SUBSET, MEM_MAP, PULL_EXISTS, MEM_GENLIST, pure_vars]
+            )
+          )
+        >- (
+          first_x_assum drule >> simp[EL_MEM, SUBSET_DEF] >> rw[] >>
+          first_x_assum drule >> simp[]
+          )
+        )
+      >- (
+        gvs[SUBSET_DEF] >> gen_tac >> strip_tac >>
+        Cases_on `tyrest` >> gvs[DISJ_IMP_THM, FORALL_AND_THM] >>
+        first_x_assum drule >> simp[]
+        )
+      ) >>
+    qpat_x_assum `get_typedef _ _ _ = _` kall_tac >>
+    qpat_x_assum `PERM _ _` kall_tac >>
+    qpat_x_assum `infer _ _ _ _ = _` kall_tac >>
+    `∀mvar. mvar ∈ domain mset ⇒ mvar < ar + SUC n` by (
+      rw[] >> last_x_assum drule >> simp[]) >>
+    last_x_assum assume_tac >>
+    ntac 4 $ last_x_assum kall_tac >>
+    rpt $ pop_assum mp_tac >>
+    map_every qid_spec_tac [`n`,`l`,`tyrest`,`asrest`,`csrest`] >>
+    Induct_on `cases` >> rw[] >> simp[]
+    >- (
+      qexistsl_tac [`[]`,`[]`,`[]`,`[]`] >> simp[assumptions_rel_def, iFunctions_def] >>
+      simp[cvars_disjoint_def, new_vars_def, list_disjoint_def, pure_vars]
+      ) >>
+    gvs[Abbr `f`] >> pairarg_tac >> gvs[] >>
+    every_case_tac >> gvs[PULL_EXISTS, EXISTS_PROD] >>
+    qmatch_asmsub_abbrev_tac `FOLDR f` >>
+    rename1 `FOLDR _ _ _ _ = SOME ((tysrest,asrest,csrest),r)` >>
+    rename1 `infer _ _ _ _ = SOME ((ty,as,cs),m)` >>
+    gvs[DISJ_IMP_THM, FORALL_AND_THM] >>
+    last_x_assum drule >> disch_then drule >> simp[] >>
+    strip_tac >> gvs[] >>
+    first_x_assum drule >> impl_tac
+    >- (rw[domain_list_insert, MEM_GENLIST] >> gvs[] >> first_x_assum drule >> simp[]) >>
+    strip_tac >> gvs[] >>
+    gvs[domain_list_insert_alt, GSYM CONJ_ASSOC, INSERT_UNION_EQ] >>
+    goal_assum $ drule_at $ Pat `LIST_REL _ _ _` >>
+    goal_assum $ drule_at $ Pat `minfer _ _ _ _ _` >>
+    qexistsl_tac [`mas::ass`,`set (MAP to_mconstraint cs) :: css`] >> simp[] >>
+    simp[PULL_EXISTS, GSYM CONJ_ASSOC, EXISTS_PROD] >>
+    goal_assum $ drule_at $ Pat `LIST_REL _ _ _` >>
+    Cases_on `ALOOKUP cdefs cn` >> gvs[inferM_rws] >> rw[] >>
+    rewrite_tac[Once $ GSYM ZIP] >> irule_at Any EQ_REFL >> simp[] >> rw[]
+    >- (
+      gvs[assumptions_rel_def, aunion_def] >> simp[PULL_FORALL] >> rpt gen_tac >>
+      DEP_REWRITE_TAC[lookup_unionWith, lookup_list_delete] >>
+      DEP_REWRITE_TAC[cj 1 unionWith_thm, cj 2 unionWith_thm] >>
+      DEP_REWRITE_TAC[cj 1 map_ok_list_delete, cj 2 map_ok_list_delete] >> simp[] >>
+      simp[Once maunion_def, FLOOKUP_FMERGE, FLOOKUP_FDIFF] >>
+      rw[] >> every_case_tac >> gvs[] >> metis_tac[wf_union, domain_union]
+      )
+    >- (
+      DEP_REWRITE_TAC[MAP2_MAP] >>
+      simp[MAP_FLAT, MAP_MAP_o, combinTheory.o_DEF, LIST_TO_SET_MAP, IMAGE_IMAGE,
+           LIST_TO_SET_FLAT, LAMBDA_PROD, IMAGE_BIGUNION] >>
+      drule LIST_TO_SET_get_assumptions >> rw[] >>
+      qpat_x_assum `MEM _ (MAP _ _)` mp_tac >> rw[MEM_MAP] >> pairarg_tac >> gvs[] >>
+      drule_all ALOOKUP_ALL_DISTINCT_MEM >> simp[]
+      )
+    >- (
+      gvs[cvars_disjoint_def] >>
+      once_rewrite_tac[CONS_APPEND] >> rewrite_tac[list_disjoint_append] >>
+      simp[MEM_MAP, EXISTS_PROD, PULL_EXISTS] >> rpt gen_tac >>
+      DEP_REWRITE_TAC[MEM_ZIP] >> DEP_REWRITE_TAC[cj 1 LENGTH_ZIP] >> simp[] >>
+      imp_res_tac LIST_REL_LENGTH >> gvs[] >> simp[PULL_EXISTS] >> rw[] >>
+      pop_assum mp_tac >> DEP_REWRITE_TAC[EL_ZIP] >> simp[] >> strip_tac >> gvs[] >>
+      irule SUBSET_DISJOINT >> goal_assum $ drule_at Any >>
+      qexists_tac `{v | ar + SUC n ≤ v ∧ v < r}` >>
+      conj_tac >- rw[DISJOINT_ALT] >> gvs[] >> rw[] >>
+      irule SUBSET_TRANS >> goal_assum $ drule_at Any >>
+      gvs[new_vars_def, BIGUNION_SUBSET, pure_vars, PULL_EXISTS] >> rw[]
+      >- (
+        simp[SUBSET_DEF] >> rw[] >> disj1_tac >> disj1_tac >>
+        gvs[IN_FRANGE_FLOOKUP, FLOOKUP_FOLDR_maunion, PULL_EXISTS,
+            GSYM CONJ_ASSOC, FLOOKUP_DEF, BIGUNION_SUBSET] >>
+        rpt $ goal_assum $ drule_at Any >> simp[EL_MEM]
+        )
+      >- (
+        simp[SUBSET_DEF] >> rw[] >> disj1_tac >> disj2_tac >>
+        simp[PULL_EXISTS] >> ntac 2 $ goal_assum drule >> simp[EL_MEM]
+        )
+      >- (
+        simp[SUBSET_DEF] >> rw[] >> disj2_tac >> simp[MEM_MAP, PULL_EXISTS] >>
+        simp[pure_vars_iFunctions, pure_vars] >>
+        simp[MEM_MAP, PULL_EXISTS] >> goal_assum drule >> simp[EL_MEM]
+        )
+      )
+    >- (
+      gvs[new_vars_def, BIGUNION_FRANGE_maunion, GSYM CONJ_ASSOC,
+          pure_vars, pure_vars_iFunctions] >> rw[] >>
+      rename1 `foo ⊆ _` >> gvs[SUBSET_DEF] >> rw[] >> first_x_assum drule >> rw[]
+      )
+    )
+  >- gvs[fail_def] (* Seq empty case *)
+  >- gvs[fail_def] (* Seq singleton case *)
+  >- gvs[fail_def] (* Seq too many args case *)
+QED
 
 val _ = export_theory();
 
